\documentclass{ximera}
\input{../../preamble.tex}
\begin{document}
\begin{exercise} \label{c4.5.1}
Consider
\begin{equation}  \label{e:Ceqn}
\frac{dX}{dt}(t) = CX(t)
\end{equation}
where
\[
C=\left(\begin{array}{cr} 2 & 3\\0& -1 \end{array}\right).
\]
Let
\[
v_1=\left(\begin{array}{c} 1\\0\end{array}\right)\AND
v_2=\left(\begin{array}{r} 1\\-1\end{array}\right),
\]
and let
\[
Y(t)=e^{2t} v_1 \AND Z(t)=e^{-t}v_2.
\]
\begin{enumeratea}
\item Show that $Y(t)$ and $Z(t)$ are solutions to \eqref{e:Ceqn}.
\item Show that $X(t)=2Y(t)-14Z(t)$ is a solution to \eqref{e:Ceqn}.
\item Use the principle of superposition to verify that
$X(t)=\alpha Y(t) + \beta Z(t)$ is a solution to \eqref{e:Ceqn}.
\item Using the general solution found in part (c), find a solution
$X(t)$ to \eqref{e:Ceqn} such that
\[
X(0) = \left(\begin{array}{r} 3\\-1\end{array}\right).
\]
\end{enumeratea}

\begin{solution}
\soln
\begin{enumeratea}
\item In order to determine that $Y(t)$ is a solution
to \eqref{e:Ceqn}, substitute $Y(t)$ into both sides of the 
equation $\frac{dX}{dt} = CX$:
\[
\frac{dY}{dt}
= \frac{d}{dt}\left(e^{2t}\vectwo{1}{0}\right)
= \frac{d}{dt}\cvectwo{e^{2t}}{0}
= \cvectwo{2e^{2t}}{0};
\]
\[
CY(t)
= \mattwo{2}{3}{0}{-1}\cvectwo{e^{2t}}{0}
= \cvectwo{2e^{2t}}{0}.
\]
Similarly, show that $Z(t)$ is a solution:
\[
\frac{dZ}{dt}
= \frac{d}{dt}\left(e^{-t}\vectwo{1}{-1}\right)
= \frac{d}{dt}\cvectwo{e^{-t}}{-e^{-t}}
= \cvectwo{-e^{-t}}{e^{-t}};
\]
\[
CZ(t)
= \mattwo{2}{3}{0}{-1}\cvectwo{e^{-t}}{-e^{-t}}
= \cvectwo{-e^{-t}}{e^{-t}}.
\]

\item Again, verify that $X(t) = 2Y(t) - 14Z(t)$ is a solution to
\eqref{e:Ceqn} by substituting into both sides of the equation and
noting that the values are equal:
\[
\frac{dX}{dt}
= \frac{d}{dt}\left(2e^{2t}\vectwo{1}{0} - 14e^{-t}\vectwo{1}{-1}\right)
= \frac{d}{dt}\cvectwo{2e^{2t} - 14e^{-t}}{14e^{-t}} 
= \cvectwo{4e^{2t} + 14e^{-t}}{-14e^{-t}};
\]
\[
CX(t) = C\left(2Y(t) - 14Z(t)\right)
= C\left(\cvectwo{2e^{2t}}{0} - \cvectwo{14e^{-t}}{-14e^{-t}}\right)
= \cvectwo{4e^{2t} + 14e^{-t}}{-14e^{-t}}.
\]

\item As demonstrated in Section~\ref{S:Superposition}, if
$Y(t)$ and $Z(t)$ are both solutions to
\eqref{e:Ceqn}, then $X(t) = \alpha Y(t) + \beta Z(t)$ is also
a solution to \eqref{e:Ceqn}.

\item  \ans 
\[
X(t) = 2e^{2t}\vectwo{1}{0} + e^{-t}\vectwo{1}{-1}.
\]

\soln Note that
\[ X(t) = \alpha Y(t) + \beta Z(t) = \alpha e^{2t}\vectwo{1}{0}
+ \beta e^{-t}\vectwo{1}{-1} \]
is a solution to \eqref{e:Ceqn}.  Substitute the value
$X(0) = (3,-1)^t$  into the equation to find a solution with that
initial condition:
\[
\vectwo{3}{-1} = X(0) = \alpha\vectwo{1}{0} +
\beta\vectwo{1}{-1}.
\]
We now have the linear system:
\[ \begin{array}{rrrrr}
3 & = & \alpha & + & \beta \\
-1 & = & & & -\beta \end{array} \]
which we can solve to find $\alpha = 2$ and $\beta = 1$.
\end{enumeratea}

\end{solution}
\end{exercise}
\end{document}
