\documentclass{ximera}
\input{../../preamble.tex}
\begin{document}
\begin{exercise} \label{c3.4.2}
Let $(x(t),y(t))$ be the solution \eqref{e:explicitsoln} of \eqref{lin2}
with initial condition $(x(0),y(0))=(x_0,y_0)$, where $x_0\neq 0 \neq y_0$.
\begin{itemize}
\item[(a)] Show that the points $(x(t),y(t))$ lie on the curve whose 
equation is:
\[
y_0^ax^d - x_0^dy^a = 0.
\]
\item[(b)] Verify that if $a=1$ and $d=2$, then the solution lies
on a parabola tangent to the $x$-axis.
\end{itemize}

\begin{solution}

The solutions $x(t)$ and $y(t)$ are:
\[
\begin{array}{rcl}
x(t) & = & x_0e^{At} \\
y(t) & = & y_0e^{Dt}\end{array}.
\]
We show that the point $(x(t),y(t))$ lies on the curve
$y_0^Ax^D - x_0^Dy^A = 0$ as follows.  Substitute the formulas for
$x(t)$ and $y(t)$ into the equation to obtain
\[
y_0^A\left(x_0e^{At}\right)^D - x_0^D\left(y_0e^{Dt}\right)^A =
x_0^Dy_0^Ae^{ADt} - x_o^Dy_0^Ae^{ADt} = 0.
\]
If $A = 1$ and $D = 2$, then the solutions lie on the curve
$0 = y_0x^2 - x_0^2y$, which can be rewritten as
$y = \dps \frac{y_0}{x_0^2}x^2$.
Since $x_0$ and $y_0$ are constants, this curve is a parabola
tangent to the $x$-axis.

\end{solution}
\end{exercise}
\end{document}
