\documentclass{ximera}
\input{../../preamble.tex}
\begin{document}

\noindent In Exercises~\ref{c12.3.4a} -- \ref{c12.3.4d} apply the
method of elimination to find the general solution of the given
system of differential equations.
\begin{exercise} \label{c12.3.4a}
$\begin{array}{rcl}
\dot{x} & = & y\\
\dot{y} & = & 2x+y
\end{array}$

\begin{solution}
\ans $X(t) = ae{2t}\vectwo{1}{2} + be^{-t}\vectwo{1}{-1}$.

\soln  The characteristic polynomial of the coefficient matrix is 
$p(\lambda) = \lambda^2-\lambda-2=(\lambda-2)(\lambda+1)$.  Therefore, 
\[
x(t) = ae^{2t}+be^{-t}.
\]
It follows from the first differential equation that 
\[
y = \dot{x} = 2ae^{2t}-be^{-t}.
\]
Therefore,
\[
X(t) = ae^{2t}\vectwo{1}{2} + be^{-t}\vectwo{1}{-1}.
\]


\end{solution}
\end{exercise}
\begin{exercise} \label{c12.3.4b}
$\begin{array}{rcl}
\dot{x} & = & x-y\\
\dot{y} & = & x+y
\end{array}$

\begin{solution}
\ans $X(t) = ae^t\cos t\vectwo{1}{1} + be^t\sin t\vectwo{1}{-1}$.

\soln  The characteristic polynomial of the coefficient matrix is 
$p(\lambda) = \lambda^2-2\lambda+2$.  The roots of $p(\lambda)$ are $1\pm i$. 
Therefore, 
\[
x(t) = ae^t\cos t+be^t\sin t.
\]
It follows from the first differential equation that 
\[
y = x-\dot{x} = e^t(a\cos t+b\sin t) - e^t(a\cos t+b\sin t-a\sin t+b\cos t)
=e^t(a\sin t-b\cos t).
\]
Therefore,
\[
X(t) = ae^t\cos t\vectwo{1}{1} + be^t\sin t\vectwo{1}{-1}.
\]


\end{solution}
\end{exercise}
\begin{exercise} \label{c12.3.4c}
$\begin{array}{rcl}
\dot{x} & = & x+y\\
\dot{y} & = & 4x-2y
\end{array}$

\begin{solution}
\ans $X(t) = ae^{2t}\vectwo{1}{1} + be^t\vectwo{1}{-4}$.

\soln  The characteristic polynomial of the coefficient matrix is 
$p(\lambda) = \lambda^2+\lambda-6=(\lambda-2)(\lambda+3)$.  Therefore, 
\[
x(t) = ae^{2t}+be^{-3t}.
\]
It follows from the first differential equation that 
\[
y =\dot{x}-x = (2ae^{2t}-3be^{-3t})-(ae^{2t}+be^{-3t}) = ae^{2t}-4be^{-3t}.
\]
Therefore,
\[
X(t) = ae^{2t}\vectwo{1}{1} + be^{-3t}\vectwo{1}{-4}.
\]


\end{solution}
\end{exercise}
\begin{exercise} \label{c12.3.4d}
$\begin{array}{rcl}
\dot{x} & = & 2x-y\\
\dot{y} & = & y
\end{array}$

\begin{solution}
\ans $X(t) = ae^{2t}\vectwo{1}{0} + be^t\vectwo{1}{1}$.

\soln  The characteristic polynomial of the coefficient matrix is 
$p(\lambda) = \lambda^2-3\lambda+2=(\lambda-2)(\lambda-1)$.  Therefore, 
\[
x(t) = ae^{2t}+be^t.
\]
It follows from the first differential equation that 
\[
y = 2x-\dot{x} = 2(ae^{2t}+be^t)-(2ae^{2t}+be^t) = be^t.
\]
Therefore,
\[
X(t) = ae^{2t}\vectwo{1}{0} + be^t\vectwo{1}{1}.
\]


\end{solution}
\end{exercise}
\end{document}
