\documentclass{ximera}
\input{../../preamble.tex}
\begin{document}


\noindent In Exercises~\ref{c13.3.2} -- \ref{c13.2.2}, use Laplace transforms 
to compute the solution to the given initial value problem.
\begin{exercise} \label{c13.3.2}
$\ddot{x} + 2\dot x +5x = 0, \quad x(0) = 2, \quad \dot{x}(0) = -6$.

\begin{solution}
\ans The solution to the initial value problem is
\[
x(t) = 2e^{-t}\cos(2t) - 2e^{-t}\sin(2t).
\]
\soln First, apply the Laplace transform to both sides of the differential
equation:
\[
0 = {\cal L}[\ddot{x}] + 2{\cal L}[\dot{x}] + 5{\cal L}[x]
= (s^2 + 2s + 5){\cal L}[x] - (2s - 2).
\]
Next, solve for ${\cal L}[x]$.  The denominator of the partial fraction
has no real roots, so complete the square, obtaining
\[
{\cal L}[x]
= \frac{2s - 2}{s^2 + 2s + 5}
= 2\frac{s - 1}{(s + 1)^2 + 4}
= 2\frac{(s + 1) - 2}{(s + 1)^2 + 4}
= 2\frac{s + 1}{(s + 1)^2 + 4} - 2\frac{2}{(s + 1)^2 + 4}.
\]
Now, let
\[
Y(s) = 2\frac{s}{s^2 + 4} - 2\frac{2}{s^2 + 4}.
\]
Then, using Table~\ref{tab:Laplist},
\[
{\cal L}^{-1}[Y(s)] = 2\cos(2t) - 2\sin(2t)
\]
and, by Proposition~\ref{prop:eHcLap1}(b),
\[
x(t) = {\cal L}^{-1}[Y(s + 1)] = e^{-1}{\cal L}^{-1}[Y(s)].
\]


\end{solution}
\end{exercise}
\begin{exercise} \label{c13.4.3a}
$\ddot x +4\dot x +20 x=0,\quad x(0)=1,\quad \dot{x}(0)=-6$.

\begin{solution}
\ans The solution to the initial value problem is
\[
x(t) = e^{-2t}\cos(4t) - e^{-2t}\sin(4t).
\]
\soln First, apply the Laplace transform to both sides of the differential
equation:
\[
0 = {\cal L}[\ddot{x}] + 4{\cal L}[\dot{x}] + 20{\cal L}[x]
= (s^2 + 4s + 20){\cal L}[x] - (s - 2).
\]
Next, solve for ${\cal L}[x]$.  The denominator of the partial fraction
has no real roots, so complete the square, obtaining
\[
{\cal L}[x]
= \frac{s - 2}{s^2 + 4s + 20}
= \frac{s - 2}{(s + 2)^2 + 16}
= \frac{(s + 2) - 4}{(s + 2)^2 + 16}
= \frac{s + 2}{(s + 2)^2 + 16} - \frac{4}{(s + 2)^2 + 16}.
\]
Now, let
\[
Y(s) = \frac{s}{s^2 + 16} - \frac{4}{s^2 + 16}.
\]
Then, using Table~\ref{tab:Laplist},
\[
{\cal L}^{-1}[Y(s)] = \cos(4t) - \sin(4t)
\]
and, by Proposition~\ref{prop:eHcLap1}(b),
\[
x(t) = {\cal L}^{-1}[Y(s + 2)] = e^{-2}{\cal L}^{-1}[Y(s)].
\]


\end{solution}
\end{exercise}
\begin{exercise} \label{c13.4.3b}
$\ddot x -6\dot x +13 x=1,\quad x(0)=0,\quad \dot{x}(0)=1$.

\begin{solution}
\ans The solution to the initial value problem is
\[
x(t) = \frac{1}{13}\left(1 + e^{3t}\cos(2t) - 8e^{3t}\sin(2t)\right).
\]
\soln First, apply the Laplace transform to both sides of the differential
equation:
\[
\frac{1}{s} = {\cal L}[1]
= {\cal L}[\ddot{x}] - 6{\cal L}[\dot{x}] + 13{\cal L}[x]
= (s^2 - 6s + 13){\cal L}[x] - 1.
\]
Next, solve for ${\cal L}[x]$ by using partial fractions, then completing
the square:
\[
\begin{array}{rcl}
{\cal L}[x] & = & \frac{s + 1}{s(s^2 - 6s + 13)} \\
& = & \frac{1}{13}\left(\frac{1}{s}\right) +
\frac{1}{13}\left(\frac{s - 19}{s^2 - 6s + 13}\right) \\
& = & \frac{1}{13}\left(\frac{1}{s} +
\frac{s - 3}{(s + 3)^2 + 4} - 8\frac{2}{(s - 3)^2 + 4}\right).
\end{array}
\]
Now, let
\[
Y(s) = \frac{s}{s^2 + 4} - 8\frac{2}{s^2 + 4}.
\]
Then, using Table~\ref{tab:Laplist},
\[
{\cal L}^{-1}[Y(s)] = \cos(2t) - 8\sin(2t)
\]
and, by Proposition~\ref{prop:eHcLap1}(b),
\[
x(t) = \frac{1}{13}\left({\cal L}^{-1}\left[\frac{1}{s}\right] +
{\cal L}^{-1}[Y(s - 3)]\right) =
\frac{1}{13}\left(1 + e^{3t}{\cal L}^{-1}[Y(s)]\right).
\]



\end{solution}
\end{exercise}
\begin{exercise} \label{c13.2.1}
$\ddot{x} + 2\dot{x} - 3x  =  1, \quad x(0) = 2, \quad \dot{x}(0) = 0$.

\begin{solution}
\ans The solution to the initial value problem is
\[
x(t) = -\frac{1}{3} + \frac{7}{12}e^{-3t} + \frac{7}{4}e^t.
\]
\soln First, apply the Laplace transform to both sides of the ordinary
differential equation:
\[
\frac{1}{s} = {\cal L}[1]
= {\cal L}[\ddot{x}] + 2{\cal L}[\dot{x}] - 3{\cal L}[x]
= (s^2 + 2s - 3){\cal L}[x] - (2s + 4).
\]
Then, use partial fractions to solve for ${\cal L}[x]$, obtaining
\[
{\cal L}[x] = \frac{\frac{1}{s} + (2s + 4)}{s^2 + 2s - 3}
= \frac{2s^2 + 4s + 1}{s(s + 3)(s - 1)}
= \frac{-\frac{1}{3}}{s} + \frac{\frac{7}{12}}{s + 3}
+ \frac{\frac{7}{4}}{s - 1}.
\]
Now compute
\[
\begin{array}{rcl}
{\cal L}^{-1}\left[\frac{-\frac{1}{3}}{s} + \frac{\frac{7}{12}}{s + 3}
+ \frac{\frac{7}{4}}{s - 1}\right]
& = & -\frac{1}{3}{\cal L}^{-1}\left[\frac{1}{s}\right]
+ \frac{7}{12}{\cal L}^{-1}\left[\frac{1}{s + 3}\right]
+ \frac{7}{4}{\cal L}^{-1}\left[\frac{1}{s - 1}\right] \\
& = & -\frac{1}{3} + \frac{7}{12}e^{-3t} + \frac{7}{4}e^t.
\end{array}
\]

\end{solution}
\end{exercise}
\begin{exercise} \label{c13.2.2}
$\ddot{x} + 2\dot{x} - 8x = e^t, \quad x(0) = 1, \quad \dot{x}(0) = 2$.

\begin{solution}
\ans The solution to the initial value problem is
$x(t) = \frac{1}{30}(35e^{2t}-6e^t+e^{-4t})$.

\soln Apply the Laplace transform to both sides of the ordinary
differential equation:
\[
\frac{1}{s-1} = {\cal L}[e^t]
= {\cal L}[\ddot{x}] + 2{\cal L}[\dot{x}] - 8{\cal L}[x]
= (s^2 + 2s - 8){\cal L}[x] - (s + 4).
\]
Then, use partial fractions to solve for ${\cal L}[x]$, obtaining
\[
{\cal L}[x] = \frac{s+4}{(s + 4)(s - 2)}
= \frac{1}{s-2} + \frac{1}{(s-1)(s-2)(s+4)}
= \frac{1}{30}\left(\frac{35}{s-2} - \frac{6}{s-1} + \frac{1}{s-4}\right).
\]
Therefore, $x(t)=\frac{1}{30}(35e^{2t}-6e^t+e^{-4t})$.


\end{solution}
\end{exercise}
\end{document}
