\documentclass{ximera}
\input{../../preamble.tex}
\begin{document}
\begin{exercise} \label{c13.1.2}
Suppose that $z(t)=ty(t)$.  Using \eqref{E:laplace} show that
\[
{\cal L}[z](s) = -\frac{\dps d}{\dps ds} {\cal L}[y](s).
\]

\begin{solution}
Compute
\[
\begin{array}{rcl}
\frac{d}{ds}{\cal L}[y](s)
& = & \frac{d}{ds}\left(\int_0^\infty e^{-st}y(t)dt\right) \\
& = & \int_0^\infty\left(\frac{d}{ds} e^{-st}y(t)dt\right) \\
& = & \int_0^\infty (-te^{-st}y(t)dt) \\
& = & -\int_0^\infty (z(t)e^{-st}dt) \\
& = & -{\cal L}[z](s)
\end{array}
\]
as desired.





\end{solution}
\end{exercise}
\end{document}
