\documentclass{ximera}

\input{../preamble.tex}

\title{Existence of Determinants}

\begin{document}
\begin{abstract}
\end{abstract}
\maketitle


\label{A:det}

The purpose of this appendix is to verify the inductive
definition of determinant \Ref{e:inductdet}. We have already
shown that if a determinant function exists, then it is unique.
We also know that the determinant function exists for $1\times
1$ matrices. So we assume by induction that the determinant function
exists for $(n-1)\times(n-1)$ matrices and prove that the
inductive definition gives a determinant function for $n\times
n$ matrices.  \index{determinant}

Recall that $A_{ij}$ is the cofactor matrix obtained from $A$ by
deleting the $i^{th}$ row and $j^{th}$ column --- so $A_{ij}$ is
an $(n-1)\times(n-1)$ matrix.  The inductive definition is:
\index{determinant!inductive formula for}
\[
D(A) = a_{11}\det(A_{11})-a_{12}\det(A_{12})+\cdots 
+(-1)^{n+1}a_{1n}\det(A_{1n}).
\] \index{cofactor}
We use the notation $D(A)$ to remind us that we have not yet
verified that this definition satisfies properties (a)-(c) of
Definition~\ref{D:determinants}.  In this appendix we verify these
properties after assuming that the inductive definition
satisfies properties (a)-(c) for $(n-1)\times (n-1)$ matrices.
For emphasis, we use the notation $\det$ to indicate the
determinant of square matrices of size less than $n$.

Property (a) is easily verified for $D(A)$ since if $A$ is lower
triangular, then
\[
D(A) = a_{11}\det(A_{11}) = a_{11}a_{22}\cdots a_{nn}
\]
by induction.

Before verifying that $D$ satisfies properties (b) and (c) of a
determinant, we prove:
\begin{lemma}
Let $E$ be a elementary row matrix and let $B$ be any $n\times
n$ matrix.   Then
\begin{equation} \label{e:proddetE}
D(EB) = D(E) D(B)
\end{equation} 
\end{lemma}

\begin{proof} We verify \Ref{e:proddetE} for each of the three types of
elementary row operations. \index{elementary row operations}

\noindent (I) Suppose that $E$ multiplies the $i^{th}$ row by a
nonzero scalar $c$.  If $i>1$, then the cofactor matrix
$(EA)_{1j}$ is obtained from the cofactor matrix $A_{1j}$ by
multiplying the $(i-1)^{st}$ row by $c$.  By induction,
$\det(EA)_{1j}= c\det(A_{1j})$ and $D(EA)=cD(A)$.  On the other
hand, $D(E)=\det(E_{11})=c$.  So \Ref{e:proddetE} is verified in
this instance.  If $i=1$, then the $1^{st}$ row of $EA$ is
$(ca_{11},\ldots,ca_{1n})$ from which it is easy to verify
\Ref{e:proddetE}.

\noindent (II) Next suppose that $E$ adds a multiple $c$ of the
$i^{th}$ row to the $j^{th}$ row.  We note that $D(E)=1$.  When
$j>1$ then $D(E)=\det(E_{11})=1$ by induction.  When $j=1$ then
$D(E)= \det(E_{11})\pm c\det(E_{1i})=\det(I_{n-1})\pm
c\det(E_{1i})$. But $E_{1i}$ is strictly upper triangular and
$\det(E_{1i})=0$.  Thus $D(E)=1$. 

If $i>1$ and $j>1$, then the result $D(EA)=D(A)=D(E)D(A)$
follows by induction.  

If $i=1$, then
\begin{eqnarray*}
D(EB) & = & b_{11}\det((EB)_{11})+\cdots+(-1)^{n+1}b_{1n}\det((EB)_{1n})\\
& = & D(B) + cD(C)
\end{eqnarray*}
where the $1^{st}$ and $i^{th}$ row of $C$ are equal.

If $j=1$, then 
\begin{eqnarray*}
D(EB) & = & (b_{11}+cb_{i1})\det(B_{11}) +\cdots+ 
(-1)^{n+1}(b_{1n}+cb_{in})\det(B_{1n})\\
& = &
\left[b_{11}\det(B_{11})+\cdots+(-1)^{n+1}b_{1n}\det(B_{1n})\right]
+ 
\\ & & 
        c\left[b_{i1}\det(B_{11})+\cdots+(-1)^{n+1}b_{i1}\det(B_{1n})\right]\\
& = & D(B) + cD(C)
\end{eqnarray*}
where the $1^{st}$ and $i^{th}$ row of $C$ are equal.  

The hardest part of this proof is a calculation that shows that
if the $1^{st}$ and $i^{th}$ rows of $C$ are equal, then
$D(C)=0$.  By induction, we can swap the $i^{th}$ row with the
$2^{nd}$.  Hence we need only verify this fact when $i=2$. 

\noindent (III) $E$ is the matrix that swaps two rows.   

As we saw earlier \Ref{e:swapdecomp}, $E$ is the product of four
matrices of types (I) and (II).  It follows that $D(E)=-1$ and
$D(EA)=-D(A)=D(E)D(A)$.  

We now verify that when the $1^{st}$ and $2^{nd}$ rows of an
$n\times n$ matrix $C$ are equal, then $D(C)=0$.  This is a
tedious calculation that requires some facility with indexes and
summations.  Rather than do this proof for general $n$, we
present the proof for $n=4$.  This case contains all of the
ideas of the general proof.  

We begin with the definition of $D(C)$
\begin{eqnarray*}
D(C) & = & c_{11}\det\left(\begin{array}{ccc} c_{22} & c_{23} & c_{24}
\\ c_{32} & c_{33} & c_{34} \\ c_{42} & c_{43} & c_{44}
\end{array}\right) 
-c_{12}\det\left(\begin{array}{ccc} c_{21} & c_{23} & c_{24}
\\ c_{31} & c_{33} & c_{34} \\ c_{41} & c_{43} & c_{44}
\end{array}\right) + \\ & &  
c_{13}\det\left(\begin{array}{ccc} c_{21} & c_{22} & c_{24}
\\ c_{31} & c_{32} & c_{34} \\ c_{41} & c_{42} & c_{44}
\end{array}\right) 
-c_{14}\det\left(\begin{array}{ccc} c_{21} & c_{22} & c_{23}
\\ c_{31} & c_{32} & c_{33} \\ c_{41} & c_{42} & c_{43}
\end{array}\right).
\end{eqnarray*}
Next we expand each of the four $3\times 3$ matrices along their
$1^{st}$ rows, obtaining
\begin{eqnarray*}
D(C) & = & 
c_{11}\left(c_{22}\det\mattwo{c_{33}}{c_{34}}{c_{43}}{c_{44}}
-c_{23}\det\mattwo{c_{32}}{c_{34}}{c_{42}}{c_{44}}
+c_{24}\det\mattwo{c_{32}}{c_{33}}{c_{42}}{c_{43}}\right)\\ & &
-c_{12}\left(c_{21}\det\mattwo{c_{33}}{c_{34}}{c_{43}}{c_{44}}
-c_{23}\det\mattwo{c_{31}}{c_{34}}{c_{41}}{c_{44}}
+c_{24}\det\mattwo{c_{31}}{c_{33}}{c_{41}}{c_{43}}\right)\\ & &
+c_{13}\left(c_{21}\det\mattwo{c_{32}}{c_{34}}{c_{42}}{c_{44}}
-c_{22}\det\mattwo{c_{31}}{c_{34}}{c_{41}}{c_{44}}
+c_{24}\det\mattwo{c_{31}}{c_{32}}{c_{41}}{c_{42}}\right)\\ & &
-c_{14}\left(c_{21}\det\mattwo{c_{32}}{c_{33}}{c_{42}}{c_{43}}
-c_{22}\det\mattwo{c_{31}}{c_{33}}{c_{41}}{c_{43}}
+c_{23}\det\mattwo{c_{31}}{c_{32}}{c_{41}}{c_{42}}\right)
\end{eqnarray*}
Combining the $2\times 2$ determinants leads to:
\begin{eqnarray*}
D(C) & = &
(c_{11}c_{22}-c_{12}c_{21})\det\mattwo{c_{33}}{c_{34}}{c_{43}}{c_{44}}
+(c_{11}c_{24}-c_{14}c_{21})\det\mattwo{c_{32}}{c_{33}}{c_{42}}{c_{43}}
\\ & & 
+(c_{12}c_{23}-c_{13}c_{22})\det\mattwo{c_{31}}{c_{34}}{c_{41}}{c_{44}}
+(c_{13}c_{21}-c_{11}c_{23})\det\mattwo{c_{32}}{c_{34}}{c_{42}}{c_{44}}
\\ & & 
+(c_{13}c_{24}-c_{14}c_{23})\det\mattwo{c_{31}}{c_{32}}{c_{41}}{c_{42}}
+(c_{14}c_{22}-c_{12}c_{24})\det\mattwo{c_{31}}{c_{33}}{c_{41}}{c_{43}}
\end{eqnarray*}
Supposing that 
\[
c_{21}=c_{11} \quad  c_{22}=c_{12} \quad c_{23}=c_{13} \quad
c_{24}=c_{14} 
\]
it is now easy to check that $D(C)=0$.

We now return to verifying that $D(A)$ satisfies properties (b)
and (c) of being a determinant.  We begin by showing that
$D(A)=0$ if $A$ has a row that is identically zero.  Suppose
that the zero row is the $i^{th}$ row and let $E$ be the matrix
that multiplies the $i^{th}$ row of $A$ by $c$.  Then $EA=A$.
Using \Ref{e:proddetE} we see that
\[
D(A)=D(EA)=D(E)D(A)=cD(A),
\]
which implies that $D(A)=0$ since $c$ is arbitrary.

Next we prove that $D(A)=0$ when $A$ is singular.  Using row 
reduction we can write
\[
A=E_s\cdots E_1R
\]
where the $E_j$ are elementary row matrices and $R$ is in
reduced echelon form\index{echelon form!reduced}.  
Since $A$ is singular, the last row of
$R$ is identically zero.  Hence $D(R)=0$ and \Ref{e:proddetE}
implies that $D(A)=0$.  

We now verify property (b).  Suppose that $A$ is singular; we
show that $D(A^t)=D(A)=0$.  Since the row rank of $A$ equals the
column rank of $A$, it follows that $A^t$ is singular when $A$
is singular.  Next assume that $A$ is nonsingular.  Then $A$ is
row equivalent to $I_n$ and we can write
\begin{equation}  \label{e:Adecomp}
A=E_s\cdots E_1,
\end{equation}
where the $E_j$ are elementary row matrices.  Since  
\[
A^t = E_1^t\cdots E_s^t
\]
and $D(E)=D(E^t)$, property (b) follows. 

We now verify property (c): $D(AB)=D(A)D(B)$.  Recall that $A$
is singular if and only if there exists a nonzero vector $v$
such that $Av=0$.  Now if $A$ is singular, then so is $A^t$.
Therefore $(AB)^t=B^tA^t$ is also singular.  To verify this
point, let $w$ be the nonzero vector such that $A^tw=0$.  Then
$B^tA^tw=0$.  Thus $AB$ is singular since $(AB)^t$ is singular.
Thus $D(AB)=0=D(A)D(B)$ when $A$ is singular.  Suppose now that
$A$ is nonsingular.  It follows that 
\[
AB = E_s\cdots E_1B.
\]
Using \Ref{e:proddetE} we see that
\[
D(AB)=D(E_s)\cdots D(E_1)D(B) = D(E_s\cdots E_1)D(B) = D(A)D(B),
\]
as desired. We have now completed the proof that a determinant
function exists. \end{proof}
\end{document}
