\documentclass{ximera}
\input{../../preamble.tex}
\begin{document}
\begin{exercise} \label{c14.6.6}
Verify that the differential equation 
\[
\frac{dx}{dt} = \frac{x}{x-t}
\]
is exact and find a solution with initial value $x(2)=3$.   Compare your 
answer with Exercise~\ref{exer:at} in Section~\ref{S:3.2}.

\begin{solution}
\ans A solution to the initial value problem is
\[
x(t) = t + \sqrt{t^2-3}.
\]

\soln Write the differential equation as $\dps\frac{dx}{dt} =
\frac{G(t,x)}{H(t,x)}$, where $G(t,x) = x$ and $H(t,x) = x - t$.  Then,
since
\[
-\frac{\partial G}{\partial x} = -1 = \frac{\partial H}{\partial t},
\]
the differential equation is exact by Proposition~\ref{prop:exact}.  Next,
we must find a function $F(t,x)$ satisfying \eqref{eq:excond}.  By integration,
obtain
\[
\Omega(t,x) = \int H(t,x)dy = \int (x - t)dx = \frac{1}{2}x^2 -tx.
\]
Then, find the function $h(t)$ such that
\[
h'(t) = -\frac{\partial}{\partial t}\Omega(t,x) - G(t,x)
= x - x = 0 .
\]
In this case, we can choose $h(t) = 0$.  Finally, compute
\[
F(t,x) = \Omega(t,x) + h(t) =  \frac{1}{2}x^2 -tx,
\]
the function satisfying \eqref{eq:excond}.  Now, substitute the initial
condition $(t,x) = (2,3)$ into $F(t,x)$, obtaining $F(2,3) = -\frac{3}{2}$.  Thus,
$x(t)$ satisfies
\[
 \frac{1}{2}x^2 -tx = -\frac{3}{2}.
\]
Solve for $x$ to find the solution to the initial value problem.  The
solution is exactly the one given in Exercise~\ref{exer:at} from
Section~\ref{S:3.2}.


\end{solution}
\end{exercise} 
\end{document}
