\documentclass{ximera}
\input{../../preamble.tex}
\begin{document}
\begin{exercise}  \label{ex:if2}
Show that the differential equation
\begin{equation} \label{Ex:nexact2}
\frac{dx}{dt} = -\frac{3x}{2t}
\end{equation}
is not exact.  Now multiply both the numerator and denominator of the 
right side of \eqref{Ex:nexact2} by $t^2x$ and show that this `new' differential
equation 
\[
\frac{dx}{dt} = -\frac{3t^2x^2}{2t^3x}
\]
is exact.  Now find all solutions to \eqref{Ex:nexact2}.

\begin{solution}
\ans The general solution is $x = \dps\pm\sqrt{\frac{C}{3t^3}}$ 
for some constant $C$.

\soln We can write the differential equation as $\dps\frac{dx}{dt} =
\frac{G(t,x)}{H(t,x)}$, where $G(t,x) = -3x$ and $H(t,x) = 2t$. 
Then we compute
\[
-\frac{\partial G}{\partial x} = 3 \AND
\frac{\partial H}{\partial t} = 2.
\]
By Proposition~\ref{prop:exact}, the differential equation is exact only
if the two sides of \eqref{eq:Gy=Hs} are equal.
On multiplying numerator and denominator by $t^2x$ we obtain
where $G(t,x) = -3t^2x^2$ and $H(t,x) = 2t^3x$. 
Then we compute
\[
-\frac{\partial G}{\partial x} = 6t^2x \AND
\frac{\partial H}{\partial t} = 6t^2x.
\]
So the new form of the differential equation is exact.

Next, we must find a function $F(t,x)$ satisfying \eqref{eq:excond}.  By
integration, obtain
\[
\Omega(t,x) = \int H(t,x)dx = \int 2t^3xdx = t^3x^2.
\]
Then, find the function $h(t)$ such that
\[
h'(t) = -\frac{\partial}{\partial t}\Omega(t,x) - G(t,x)
= 6t^2x^2.
\]
In this case, we can choose 
\[
h(t) =  2t^3x^2.  
\]
Finally, compute
\[
F(t,x) = \Omega(t,x) + h(t) = 3t^3x^2,
\]
the function satisfying \eqref{eq:excond}.  The general solution is found by 
solving $F=C$ for $x$; that is, solving
\[
3t^3x^2 = C.
\]

\end{solution}
\end{exercise}
\end{document}
