\documentclass{ximera}
\input{../../preamble.tex}
\begin{document}
\begin{exercise} \label{c4.4.1}
Consider the homogeneous linear equation
\[
x+y+z = 0
\]
\begin{enumerate}
\item[(a)]  Write all solutions to this equation as a general
superposition of a pair of vectors $v_1$ and $v_2$.
\item[(b)]  Write all solutions as a general superposition of
a second pair of vectors $w_1$ and $w_2$.
\end{enumerate}

\begin{solution}

(a) \ans All solutions can be written as a superposition of the vectors
\[
v_1 = \vecthree{-1}{1}{0} \AND v_2 = \vecthree{-1}{0}{1}.
\]

\soln The equation $x + y + z = 0$ is a linear system of three variables
in one equation.  If we consider $y$ and $z$ to be free variables, then
every solution to the system has the form
\[
\vecthree{x}{y}{z} = \left(\begin{array}{c} -y - z \\ y \\
z \end{array}\right) = y\vecthree{-1}{1}{0} +
z\vecthree{-1}{0}{1}.
\]

(b) \ans All solutions can be written as a superposition
of the second pair of vectors
\[
w_1 = \vecthree{1}{0}{-1} \AND w_2 = \vecthree{0}{1}{-1}.
\]

\soln Write the same linear system, but this time consider $x$ and $y$
to be free variables.  In this case, every solution has the form:
\[
\vecthree{x}{y}{z} = \left(\begin{array}{c} x \\ y \\
-x - y \end{array}\right) = x\vecthree{1}{0}{-1} +
z\vecthree{0}{1}{-1}.
\]

\end{solution}
\end{exercise}
\end{document}
