\documentclass{ximera}
\input{../../preamble.tex}
\begin{document}
\begin{exercise}  \label{Ex:cont}
Consider the function
\[
z(t) = H_1(t)(1-\cos(2(t-1))) = \left\{
\begin{array}{cl} 0 & t \leq 1 \\ 1-\cos(2(t-1)) & t > 1. \end{array}\right.
\]
Show that $z(t)$ is continuous at $t=1$ by verifying that 
\[
\lim_{t\to 1^+}z(t) = \lim_{t\to 1^-}z(t).
\]
Show that $z(t)$ is differentiable and that $\dot{z}(1)=0$ by verifying that 
\[
\lim_{h\to 0^+} \frac{z(1+h)-z(1)}{h} = 0 = 
\lim_{h\to 0^-} \frac{z(1+h)-z(1)}{h}
\]

\begin{solution}
Verify that the equality holds by substituting $z(t)$ into
both sides:
\[
\begin{array}{rcl}
\dps \lim_{t \rightarrow 1^{+}}z(t) & = &
\dps \lim_{t \rightarrow 1^{+}}(1 - \cos(2(t - 1))) = 1 - \cos(0) = 0. \\
\dps \lim_{t \rightarrow 1^{-}}z(t) & = &
\dps \lim_{t \rightarrow 1^{-}}(0) = 0.
\end{array}
\]
So $z(t)$ is continuous.  Similarly, verify that $z(t)$ is differentiable
by substituting $z(t)$ into both sides of the equation, then using
L'H\^{o}spital's rule:
\[
\begin{array}{rcl}
\dps \lim_{h \rightarrow 0^{+}}\frac{z(1 + h) - z(1)}{h}
& = & \dps \lim_{h \rightarrow 0^{+}}\frac{(1 - \cos(2h)) - 0}{h}
= \dps \lim_{h \rightarrow 0^{+}}2\sin(2h) = 0. \\
\dps \lim_{h \rightarrow 0^{-}}\frac{z(1 + h) - z(1)}{h}
& = & \dps \lim_{h \rightarrow 0^{-}}\frac{0}{h} = 0.
\end{array}
\]

\end{solution}
\end{exercise}
\end{document}
