\documentclass{ximera}
\input{../../preamble.tex}
\begin{document}
\begin{exercise} \label{c13.4.2}
Reconfirm that the solution of the initial value problem
\[
\ddot x + 4 x=H_1(t),\quad x(0)=1,\quad \dot x(0)=0
\]
is given by
\[
x(t)=\frac{1}{4}H_1(t)(1-\cos(2(t-1))) + \cos(2t).
\]
Use the methods of Chapter \ref{C:LDE} and proceed as follows:
\begin{itemize}
\item[(a)] Find the solution $x_1(t)$ of the initial value problem
\[
\ddot x + 4 x=0,\quad x(0)=1,\quad \dot x(0)=0
\]
on the time interval $t\in[0,1]$.
\item[(b)] Find the general solution $x_2(t)$ of the second order
differential equation $\ddot x + 4 x=1$.
\item[(c)] Adjust the parameters in $x_2(t)$ such that the function
\[
x(t)=\left\{ \begin{array}{l} x_1(t)\quad t\in[0,1]\\
x_2(t) \quad t>1 \end{array}\right.
\]
is differentiable at $t=1$.
\end{itemize}

\begin{solution}

(a) Let $p(D) = D^2 + 4$.  Then the characteristic polynomial of
$p(D)$ has eigenvalues $\lambda = \pm 2i$, and the general solution to
$p(D)x = 0$ is
\[
x(t) = \alpha_1\cos(2t) + \alpha_2\sin(2t).
\]
Substitute the initial conditions into $x(t)$, obtaining
\[
1 = x(0) = \alpha_1 \AND
0 = \dot{x}(0) = \alpha_2.
\]
Thus,
\[
x_1(t) = \cos(2t).
\]

(b) Let $g(t) = 1$ and use the method of undetermined coefficients.
\paragraph{Step 1.} An annihilator for $g(t)$ is $q(D) = D$, since
the characteristic polynomial of $q(D)$ has eigenvalue $\lambda = 0$.

\paragraph{Step 2.} The eigenvalues of $p(D)$ are distinct from that
of $q(D)$, so the trial space is simply the solution space of $q(D)$,
which is $y(t) = c_1$.

\paragraph{Step 3.} Substitute $y(t)$ into $p(D)x = g(t)$, obtaining
\[
4c_1 = 1.
\]
So, the general solution to $\ddot{x} + 4x = 1$ is
\[
x_2(t) = \alpha_1\cos(2t) + \alpha_2\sin(2t) + \frac{1}{4}.
\]

(c) In order for $x(t)$ to be continuous at $t = 1$,
\[
\dps\lim_{t \rightarrow 1^{-}} x(t) = x_1(1) = \cos(2)
\]
must equal
\[
\dps\lim_{t \rightarrow 1^{+}} x(t) = x_2(1) =
\alpha_1\cos(2) + \alpha_2\sin(2) + \frac{1}{4}.
\]
So
\begin{equation} \label{ex:13.4.2a}
\cos(2)\alpha_1 + \sin(2)\alpha_2 = \cos(2) - \frac{1}{4}.
\end{equation}
In order for $x(t)$ to be differentiable at $t = 1$,
\[
\dps\lim_{h \rightarrow 0^{-}} \frac{x(1 + h) - x(1)}{h} =
\frac{dx_1}{dt}(1) = -2\sin(2)
\]
must equal
\[
\dps\lim_{h \rightarrow 0^{+}} \frac{x(1 + h) - x(1)}{h} =
\frac{dx_2}{dt}(1) = -2\alpha_1\sin(2) + 2\alpha_2\cos(2).
\]
So
\begin{equation} \label{ex:13.4.2b}
-2\sin(2)\alpha_1 + 2\cos(2)\alpha_2 = -2\sin(2).
\end{equation}
Solve \eqref{ex:13.4.2a} and \eqref{ex:13.4.2b} to find that $x(t)$ is
differentiable when $\alpha_1 = 1 - \frac{1}{4}\cos(2)$ and $\alpha_2
= -\frac{1}{4}\sin(2)$.  Substituting these values into $x_2(t)$ and
using trigonometric identities, we obtain
\[
\begin{array}{rcl}
x_1(t) & = & \cos(2t) \\
x_2(t) & = & \frac{1}{4}(1 - \cos(2(t - 1))) + \cos(2t)
\end{array}
\]
confirming the given solution to the initial value problem.











\end{solution}
\end{exercise}
\end{document}
