\documentclass{ximera}
\input{../../preamble.tex}
\begin{document}
\begin{computerExercise} \label{c3.3.7}
Let $x(t)$ be a solution to the initial value problem
\begin{eqnarray*}
\dot{x} & = & g(x) \\
x(0) & = & x_0.
\end{eqnarray*}
Let $y(t)=x(-t)$.  Show that $y(t)$ is a solution to the
initial value problem
\begin{eqnarray*}
\dot{y} & = & -g(y) \\
y(0) & = & x_0.
\end{eqnarray*}
(Thus, to integrate the solution $x(t)$ backwards in time is the
same as solving the differential equation $\dot{y}  =  -g(y)$
forward in time.)

\begin{solution}

In order to show that $y(t)$ is a solution to the initial value problem
\[
\begin{array}{rcl}
\dot{y} & = & -g(y) \\
y(0) & = & x_0\end{array}
\]
we must show that both of these conditions are valid for $y$.  Recall that
$y(t) = x(-t)$ where $x(t)$ satisfies the initial value problem
\[ \begin{array}{rcl}
\dot{x} & = & g(x) \\
x(0) & = & x_0.\end{array} \]

The chain rule implies
\[ \dot{y} = \frac{d}{dt}[y(t)] = \frac{d}{dt}[x(-t)] =
-\frac{dx}{dt}(-t) = -g(x(-t)) = -g(y(t)). \]
It follows that $\dot y = -g(y)$.
In addition,
\[ y(0) = x(-0) = x(0) = x_0, \]
so $y(t)$ is indeed a solution to the given initial value problem.

\end{solution}
\end{computerExercise}
\end{document}
