\documentclass{ximera}
\input{../../preamble.tex}
\begin{document}




\noindent In Exercises~\ref{c12.2.a} -- \ref{c12.2.d} rewrite the given
higher order equation as a first order system.
\begin{exercise} \label{c12.2.a}
$\ddot{x}+5\dot{x}+x = 0$

\begin{solution}
\ans $\left\{\begin{array}{rcl} \dot{x} & = & y \\
\dot{y} & = & -x-5y. \end{array}\right.$

\soln  Let $y = \dot{x}$.  Then $\dot{y}+5y+x=0$.


\end{solution}
\end{exercise}
\begin{exercise} \label{c12.2.b}
$\ddot{x}-10x = 0$

\begin{solution}
\ans $\left\{\begin{array}{rcl} \dot{x} & = & y \\
\dot{y} & = & 10x. \end{array}\right.$

\soln  Let $y = \dot{x}$.  Then $\dot{y}-10x=0$.


\end{solution}
\end{exercise}
\begin{exercise} \label{c12.2.c}
$\frac{d^3x}{dt^3}-4\frac{d^2x}{dt^2}-10x = 0$

\begin{solution}
\ans $\left\{\begin{array}{rcl} \dot{x} & = & y \\
\dot{y} & = & z\\
\dot{z} & = & 10x+4z. \end{array}\right.$

\soln  Let $y = \dot{x}$ and $z=\dot{y}=\ddot{x}$.  Then 
$\dot{z}-4z-10x=0$.


\end{solution}
\end{exercise}
\begin{exercise} \label{c12.2.d}
$\frac{d^4x}{dt^4}+2\frac{d^2x}{dt^2}-3\frac{dx}{dt}-2x = 0$

\begin{solution}
\ans $\left\{\begin{array}{rcl} \dot{x} & = & y \\
\dot{y} & = & z\\
\dot{z} & = & u\\
\dot{u} & = & 2x+3y-2z. \end{array}\right.$

\soln  Let $y = \dot{x}$, $z=\dot{y}=\ddot{x}$ and $u=\dot{z}$.  Then 
$\dot{u}+2z-3y-2x=0$.

\end{solution}
\end{exercise}
\end{document}
