\documentclass{ximera}

\input{../preamble.tex}

\title{The Cayley Hamilton Theorem}

\begin{document}
\begin{abstract}
\end{abstract}
\maketitle

\label{S:6.6}
%\index{closed form solution}\index{matrix!exponential!computation}

The Jordan normal form theorem for real $2\times 2$ matrices states that 
every $2\times 2$ matrix is similar to one of the matrices in Table~\ref{T:3sys}.
We use this theorem to prove the Cayley Hamilton theorem 
\index{Cayley Hamilton theorem} for $2\times 2$ 
matrices and then use the Cayley Hamilton theorem to present another method 
for computing solutions to planar linear systems of differential equations in the 
case of real equal eigenvalues.


The Cayley Hamilton theorem states that a matrix satisfies its own
characteristic polynomial.  More precisely:
\begin{theorem}[Cayley Hamilton Theorem] \label{T:CH2}
Let $A$ be a $2\times 2$ matrix and let
\[
p_A(\lambda) = \lambda^2 + a\lambda + b
\]
be the characteristic polynomial\index{characteristic polynomial} of $A$.  Then
\[
p_A(A) = A^2 + aA + bI_2 = 0.
\]
\end{theorem}

\begin{proof}  Suppose $B=P\inv AP$ and $A$ are similar matrices.  We claim that
if $p_A(A)=0$, then $p_B(B)=0$.  To verify this claim, recall from
Lemma~\ref{L:simdettr} that $p_A=p_B$ and calculate
\begin{align*}
  p_B(B) &= p_A(P\inv AP) = (P\inv AP)^2 + aP\inv AP + bI_2 \\
  &= P\inv p_A(A)P= 0.
\end{align*}
Theorem~\ref{T:putinform} classifies $2\times 2$ matrices up to similarity.
Thus, we need only verify this theorem for the matrices
\begin{align*}
C &=  \mattwoc{\lambda_1}{0}{0}{\lambda_2},
D &=  \mattwo{\sigma}{-\tau}{\tau}{\sigma},
E &=  \mattwoc{\lambda_1}{1}{0}{\lambda_1},
\end{align*}
that is, we need to verify that
\[
p_C(C) = 0 \qquad p_D(D)=0 \qquad p_E(E)=0.
\]

Using the fact that $p_A(\lambda)=\lambda^2-\trace(A)\lambda+\det(A)$, we see
that
\begin{eqnarray*}
p_C(\lambda) & = & (\lambda-\lambda_1)(\lambda-\lambda_2) \\
p_D(\lambda) & = & \lambda^2 - 2\sigma \lambda + (\sigma^2+\tau^2) \\
p_E(\lambda) & = & (\lambda-\lambda_1)^2.
\end{eqnarray*}
It now follows that
\begin{align*}
  p_C(C) &= (C-\lambda_1I_2)(C-\lambda_2I_2) 
           \\
&=\mattwoc{0}{0}{0}{\lambda_2-\lambda_1}\mattwoc{\lambda_1-\lambda_2}{0}{0}{0} \\
&=0,
\end{align*}
and
\begin{align*}
p_D(D) &=
\mattwoc{\sigma^2-\tau^2}{-2\sigma\tau}{2\sigma\tau}{\sigma^2-\tau^2} -\\
       &\quad 2\sigma \mattwo{\sigma}{-\tau}{\tau}{\sigma} + \\
  &\quad (\sigma^2+\tau^2)\mattwo{1}{0}{0}{1} = 0,
\end{align*}
and
\[
p_E(E) = (E-\lambda_1I_2)^2 = \mattwo{0}{1}{0}{0}^2 = 0.
\]
\end{proof}


\subsection*{The Example with Equal Eigenvalues Revisited}

When the eigenvalues $\lambda_1=\lambda_2$, the closed form solution of 
$\dot{X} = CX$ is a straightforward formula
\begin{equation}  \label{E:exeq}
X(t) = e^{\lambda_1 t}(I_2 + tN)
\end{equation}
where $N = C - \lambda_1I_2$.

Note that when using \eqref{E:exeq}, it is not necessary to 
compute the eigenvector or generalized eigenvector of $C$, 
and this is a substantial simplification.  

\subsubsection*{Verification of \protect\eqref{E:exeq}}

We use the Cayley-Hamilton theorem to verify \eqref{E:exeq} as follows.
Specifically, since $C$ is assumed to have a double eigenvalue $\lambda_1$, it follows that
\[
N = C - \lambda_1 I_2
\]
has zero as a double eigenvalue.  Hence, the characteristic polynomial
$p_N(\lambda) = \lambda^2$ and the Cayley Hamilton theorem implies that
$N^2=0$.  Therefore,
\[
CX(t) = e^{\lambda_1t}C(I_2+tN)X_0 = e^{\lambda_1t}(\lambda_1 I_2+N)(I_2+tN)X_0 
\]
Thus, using $N^2=0$, we see that 
\[
CX(t) = e^{\lambda_1t} (\lambda_1 I_2+t\lambda_1 N + N)X_0  =\dot{X}(t),
\]
as desired

%As observed in Section~\ref{S:Matrixexp} Exercise~\ref{c6.3.14} there is a similar formula in the case that the eigenvales are real and unequal; namely, \begin{equation}  \label{E:exdist2} e^{tC} = \frac{1}{\lambda_2-\lambda_1}\left(e^{\lambda_1 t}(C-\lambda_2I_2) - e^{\lambda_2 t}(C-\lambda_1I_2)\right).\end{equation}
%Note that the computation of the eigenvectors of $C$ is also not needed here.


Let us reconsider the system of differential equations \eqref{e:shearexample}
\[
\frac{dX}{dt} = \mattwo{1}{-1}{9}{-5} X = CX
\]
with initial value
\[
X_0 = \vectwo{2}{3}.
\]
The eigenvalues of $C$ are real and equal to $\lambda_1=-2$.

We may write
\[
C = \lambda_1 I_2 + N = -2I_2+N,
\]
where
\[
N = \mattwo{3}{-1}{9}{-3}.
\]
It follows from \eqref{E:exeq} that
\begin{equation}  \label{e:solntob}
e^{tC} =  e^{-2t}\left(I_2+t\mattwo{3}{-1}{9}{-3}\right)
= e^{-2t}\mattwoc{1+3t}{-t}{9t}{1-3t}.
\end{equation}
Hence the solution to the initial value problem is:
\begin{align*}
X(t) &= e^{tC}X_0 = e^{-2t}\mattwoc{1+3t}{-t}{9t}{1-3t}\vectwo{2}{3} \\
  &= e^{-2t}\vectwo{2+3t}{3+9t}.
\end{align*}




\EXER

\TEXER

\begin{exercise} \label{c6.6.2}
Solve the initial value problem
\[
\frac{dX}{dt} = \mattwo{0}{1}{-2}{3} X
\]
where $X(0)=(2,1)^t$.

\begin{solution}

\ans The solution to the given initial value problem with $X(0) = (2,1)^t$
is
\[
X(t) = -3e^t\vectwo{1}{1} + e^{2t}\vectwo{1}{2}
= \cvectwo{e^{2t} - 3e^t}{2e^{2t} - 3e^t}.
\]

\soln Let \[ C = \mattwo{0}{1}{-2}{3}. \]
Then the solution to the system is $X(t) = e^{tC}X_0$, where
$X_0 = X(0) = (2,1)^t$.
To find $e^{tC}$, first find the eigenvalues of $C$ by solving
\[
0 = \lambda^2 - \trace(C) + \det(C) = (\lambda - 1)(\lambda - 2).
\]
The eigenvalues are $\lambda_1 = 1$ and $\lambda_2 = 2$.  We can
then find $e^{tC}$ using \eqref{E:exdist}:
\[
\begin{array}{rcl}
e^{tC} & = & \frac{1}{\lambda_2 - \lambda_1}(e^{\lambda_1 t}(C -
\lambda_2 I_2) - e^{\lambda_2 t}(C - \lambda_1 I_2)) \\
& = & e^t\left(\mattwo{0}{1}{-2}{3} - \mattwo{2}{0}{0}{2}\right) -
e^{2t}\left(\mattwo{0}{1}{-2}{3} - \mattwo{1}{0}{0}{1}\right) \\
& = &
e^t\mattwo{-2}{1}{-2}{1} - e^{2t}\mattwo{-1}{1}{-2}{2}.
\end{array}
\]
So, we can now compute
\[
X(t) = e^{tC}X_0
= \left(e^t\mattwo{-2}{1}{-2}{1} -
e^{2t}\mattwo{-1}{1}{-2}{2}\right)\vectwo{2}{1}.
\]
Complete the matrix multiplication to obtain $X(t)$.

\end{solution}
\end{exercise}

\begin{exercise} \label{c6.6.3}
Find all solutions to the linear system of ODEs
\[
\frac{dX}{dt} = \mattwo{-2}{4}{-1}{1} X.
\]

\begin{solution}

\ans The general solution is
\[
X(t) = e^{-\frac{1}{2}t}\cmattwo{\cos\left({\frac{\sqrt{7}}{2}t}\right) -
\frac{3}{2\sqrt{7}}\sin\left({\frac{\sqrt{7}}{2}t}\right)}
{\frac{4}{\sqrt{7}}\sin\left({\frac{\sqrt{7}}{2}t}\right)}
{-\frac{1}{\sqrt{7}}\sin\left({\frac{\sqrt{7}}{2}t}\right)}
{\cos\left({\frac{\sqrt{7}}{2}t}\right) +
\frac{3}{2\sqrt{7}}\sin\left({\frac{\sqrt{7}}{2}t}\right)}X(0).
\]

\soln Let
\[
C = \mattwo{-2}{4}{-1}{1}.
\]
Then the solution to the system is $X(t) = e^{tC}X_0$, where
$X_0 = X(0)$ is the initial condition of the system.
Find the eigenvalues of $C$ by solving
\[
0 = \lambda^2 - \trace(C) + \det(C) = \lambda^2 + \lambda + 2.
\]
The eigenvalues are $\lambda_1 = \frac{1}{2}(-1 + \sqrt{7}i)$ and
$\lambda_2 = \frac{1}{2}(-1 - \sqrt{7}i)$.  Find $e^{tC}$ using
\eqref{E:exdist}:
\[
e^{tC} = \frac{1}{\lambda_2 - \lambda_1}(e^{\lambda_1 t}(C -
\lambda_2 I_2) - e^{\lambda_2 t}(C - \lambda_1 I_2)).
\]
Since the scalar
\[
\frac{1}{\lambda_2 - \lambda_1} = -\frac{1}{2\sqrt{7}}i
\]
is purely
imaginary, we need compute only the imaginary parts of
$e^{\lambda_1 t}(C - \lambda_2 I_2)$ and $e^{\lambda_2 t}(C - \lambda_1 I_2)$
to obtain the real solution to the differential equation $X(t) = e^{tC}X_0$.
So, compute
\[
\begin{array}{rcl}
e^{\lambda_1 t}(C - \lambda_2 I_2)
& = & e^{-\frac{1}{2}t}e^{\frac{\sqrt{7}}{2}it}
\left(\mattwo{-2}{4}{-1}{1} - \cmattwo{-\frac{3}{2} - \frac{\sqrt{7}}{2}i}
{0}{0}{-\frac{3}{2} - \frac{\sqrt{7}}{2}i}\right) \\
& = & e^{-\frac{1}{2}t}\left(\cos\left(\frac{\sqrt{7}}{2}t\right) +
i\sin\left(\frac{\sqrt{7}}{2}t\right)\right)
\cmattwo{-\frac{3}{2} + \frac{\sqrt{7}}{2}i}{4}{-1}{\frac{3}{2} +
\frac{\sqrt{7}}{2}i}.
\end{array}
\]
The imaginary part of this product is
\[
ie^{-\frac{1}{2}t}\cmattwo{-\frac{3}{2}\sin\left(\frac{\sqrt{7}}{2}
t\right) + \frac{\sqrt{7}}{2}\cos\left(\frac{\sqrt{7}}{2}t\right)}
{4\sin\left(\frac{\sqrt{7}}{2}t\right)}{-\sin\left(\frac{\sqrt{7}}{2}t\right)}
{\frac{3}{2}\sin\left(\frac{\sqrt{7}}{2}
t\right) + \frac{\sqrt{7}}{2}\cos\left(\frac{\sqrt{7}}{2}t\right)}.
\]
Then compute
\[
\begin{array}{rcl}
e^{\lambda_2 t}(C - \lambda_1 I_2)
& = & e^{-\frac{1}{2}t}e^{-\frac{\sqrt{7}}{2}it}
\left(\mattwo{-2}{4}{-1}{1} - \cmattwo{-\frac{3}{2} + \frac{\sqrt{7}}{2}i}
{0}{0}{-\frac{3}{2} + \frac{\sqrt{7}}{2}i}\right) \\
& = & e^{-\frac{1}{2}t}\left(\cos\frac{\sqrt{7}}{2}t -
i\sin\frac{\sqrt{7}}{2}t\right)
\cmattwo{-\frac{3}{2} - \frac{\sqrt{7}}{2}i}{4}{-1}{\frac{3}{2} -
\frac{\sqrt{7}}{2}i}.
\end{array}
\]
The imaginary part of this product is
\[
ie^{-\frac{1}{2}t}\cmattwo{\frac{3}{2}\sin\left(\frac{\sqrt{7}}{2}
t\right) - \frac{\sqrt{7}}{2}\cos\left(\frac{\sqrt{7}}{2}t\right)}
{-4\sin\left(\frac{\sqrt{7}}{2}t\right)}{\sin\left(\frac{\sqrt{7}}{2}t\right)}
{-\frac{3}{2}\sin\left(\frac{\sqrt{7}}{2}
t\right) - \frac{\sqrt{7}}{2}\cos\left(\frac{\sqrt{7}}{2}t\right)}.
\]

Thus, the general solution is
\[
X(t) = \frac{1}{2\sqrt{7}}
e^{-\frac{1}{2}t}\cmattwo{-3\sin\left(\frac{\sqrt{7}}{2}t\right) +
\sqrt{7}\cos\left(\frac{\sqrt{7}}{2}t\right)}
{8\sin\left(\frac{\sqrt{7}}{2}t\right)}{-2\sin\left(\frac{\sqrt{7}}{2}t\right)}
{3\sin\left(\frac{\sqrt{7}}{2}t\right) +
\sqrt{7}\cos\left(\frac{\sqrt{7}}{2}t\right)}X_0.
\]


\end{solution}
\end{exercise}

\begin{exercise} \label{c6.6.4}
Solve the initial value problem
\[
\frac{dX}{dt} =  \mattwo{2}{1}{-2}{0}X
\]
where $X(0)=(1,1)^t$.

\begin{solution}

\ans The solution to the initial value problem $X(0) = (1,1)^t$ is:
\[
X(t) = e^t\vectwo{2\sin{t} + \cos{t}}{-3\sin{t} + \cos{t}}.
\]

\soln Let
\[
C = \mattwo{2}{1}{-2}{0}.
\]
Then the solution to the system is $X(t) = e^{tC}X_0$, where
$X_0 = X(0)$ is the initial condition of the system.
Find the eigenvalues of $C$ by solving
\[
0 = \lambda^2 - \trace(C) + \det(C) = \lambda^2 - 2\lambda + 2.
\]
So the eigenvalues of $C$ are $\lambda_1 = 1 + i$ and $\lambda_2 = 1 - i$.
We can then find $e^{tC}$ using 
\eqref{E:exdist}:
\[
e^{tC} = \frac{1}{\lambda_2 - \lambda_1}(e^{\lambda_1 t}(C -
\lambda_2 I_2) - e^{\lambda_2 t}(C - \lambda_1 I_2)).
\]
Since the scalar
\[
\frac{1}{\lambda_2 - \lambda_1} = -\frac{1}{2}i
\]
is purely imaginary, we need compute only the imaginary parts of
$e^{\lambda_1 t}(C - \lambda_2 I_2)$ and $e^{\lambda_2 t}(C - \lambda_1 I_2)$
to obtain the real solution to the differential equation $X(t) = e^{tC}X_0$.
So, compute
\[
\begin{array}{rcl}
e^{\lambda_1 t}(C - \lambda_2 I_2)
& = & e^{t}e^{it}\left(\mattwo{2}{1}{-2}{0} - \cmattwo{1 - i}{0}{0}{1 - i}
\right) \\
& = & e^{t}(\cos t + i\sin t)\cmattwo{1 + i}{1}{-2}{-1 + i}.
\end{array}
\]
The imaginary part of this product is
\[
ie^t\cmattwo{\sin t + \cos t}{\sin t}{-2\sin t}{-\sin t + \cos t}.
\]
Then compute
\[
\begin{array}{rcl}
e^{\lambda_2 t}(C - \lambda_1 I_2)
& = & e^{t}e^{-it}\left(\mattwo{2}{1}{-2}{0} - \cmattwo{1 + i}{0}{0}{1 + i}
\right) \\
& = & e^{t}(\cos t - i\sin t)\cmattwo{1 - i}{1}{-2}{-1 - i}.
\end{array}
\]
The imaginary part of this product is
\[
ie^t\cmattwo{-\sin t - \cos t}{-\sin t}{2\sin t}{\sin t - \cos t}.
\]
Thus, the solution to the given initial value problem is
\[
X(t) = e^{tC}X_0 =
\frac{1}{2}\cmattwo{2\sin t + 2\cos t}{2\sin t}{-4\sin t}{-2\sin t + 2\cos t}
\vectwo{1}{0}.
\]
Complete the matrix multiplication to obtain $X(t)$.


\end{solution}
\end{exercise}

\begin{exercise}  \label{c6.CH}
Let $A$ be a $2\times 2$ matrix.  Show that
\[
A^2 = \trace(A)A-\det(A)I_2.
\]

\begin{solution}
For any $2 \times 2$ matrix $A$, the characteristic
polynomial is
\[
p_A(\lambda) = \lambda^2 - \trace(A)\lambda + \det(A).
\]
By the Cayley-Hamilton Theorem (Theorem~\ref{T:CH2}), a $2 \times 2$
matrix satisfies its own characteristic polynomial.  Thus,
\[
p_A(A) = A^2 - \trace(A)A + \det(A)I_2 = 0,
\]
or $A^2 = \trace(A)A - \det(A)I_2$.



\end{solution}
\end{exercise}



\end{document}
