\documentclass{ximera}
\input{../../preamble.tex}
\begin{document}


\noindent In Exercises~\ref{c6.1.1a} -- \ref{c6.1.1d}, consider the system of
differential equations
\begin{equation} \label{E:c6.1.1}
\begin{array}{rcr}
\frac{dx}{dt}  & = & -y \\
\frac{dy}{dt}  & = &  x.
\end{array}
\end{equation}
\begin{exercise} \label{c6.1.1a}
Show that $(x_1(t),y_1(t)) = (\cos t,\sin t)$ is a solution to \eqref{E:c6.1.1}.

\begin{solution}

Solve by evaluation:
$(x_1(t),y_1(t)) = (\cos t, \sin t)$
is a solution because
\[ \begin{array}{ccccccc}
\frac{dx_1}{dt}(t) & = & \frac{d}{dt}(\cos t) & = & -\sin t & = & -y_1(t)
\\ \frac{dy_1}{dt}(t) & = & \frac{d}{dt}(\sin t) & = & \cos t & = & x_1(t).
\end{array}. \]

\end{solution}
\end{exercise}
\begin{exercise} \label{c6.1.1b}
Show that $(x_2(t),y_2(t)) = (-\sin t,\cos t)$ is a solution to \eqref{E:c6.1.1}.

\begin{solution}
To show that $(x_2(t),y_2(t)) = (-\sin t, \cos t)$
is a solution, calculate $v_1 = (x_1(0),y_1(0))$ and
$v_2 = (x_2(0),y_2(0))$, obtaining
\[
\begin{array}{ccccl}
v_1 = (x_1(0),y_1(0) & = & (\cos 0,\sin 0) & = & (1,0) \\
v_2 = (x_2(0),y_2(0) & = & (-\sin 0,\cos 0) & = & (0,1).
\end{array}
\]

\end{solution}
\end{exercise}
\begin{exercise} \label{c6.1.1c}
Using Exercises~\ref{c6.1.1a} and \ref{c6.1.1b}, find a solution $(x(t),y(t))$
to \eqref{E:c6.1.1} that satisfies $(x(0),y(0)) = (0,1)$.

\begin{solution}

If $(x(0),y(0)) = (0,1) = v_2$, then Theorem~\ref{T:solvends} states
that the solution is
\[
(x(t),y(t)) = (x_2(t),y_2(t)) = (-\sin t,\cos t).
\]

\end{solution}
\end{exercise}
\begin{exercise} \label{c6.1.1d}
Using Exercises~\ref{c6.1.1a} and \ref{c6.1.1b}, find a solution $(x(t),y(t))$
to \eqref{E:c6.1.1} that satisfies $(x(0),y(0)) = (1,1)$.

\begin{solution}

If $(x(0),y(0)) = (1,1) = v_1 + v_2$, then
\[
(x(t),y(t)) = (x_1(t),y_1(t)) + (x_2(t),y_2(t)) =
(\cos t - \sin t, \cos t + \sin t).
\]

\end{solution}
\end{exercise}
\end{document}
