\documentclass{ximera}
\input{../../preamble.tex}
\begin{document}

\noindent In Exercises \ref{c13.1.0A} -- \ref{c13.1.0B} use partial fractions
to find a function $x(t)$ whose Laplace transform is the given function
$Y(s)$.  {\bf Hint:}  In your calculations, you may use the result of 
Exercise~\ref{Ex:pf}.
\begin{exercise} \label{c13.1.0A}
$Y(s) = \dps\frac{1}{s^2-4s+3}$.

\begin{solution}
\ans $\dps x(t) = \frac{1}{2}(e^{3t}-e^t)$.

\soln $\dps\frac{1}{s^2-4s+3} = \frac{1}{(s-3)(s-1)} =
\frac{1}{2}\left(\frac{1}{s-3} - \frac{1}{s-1}\right)$.


\end{solution}
\end{exercise}
\begin{exercise} \label{c13.1.0B}
$Y(s) = \dps\frac{s-1}{s^2+5s+6}$.

\begin{solution}
\ans $\dps x(t) = 4e^{-3t}-3e^{-2t}$.

\soln $\dps\frac{s-1}{s^2+5s+6} = \frac{s-1}{(s+3)(s+2)} =
\frac{4}{s+3} - \frac{3}{s+2}$.

\end{solution}
\end{exercise}
\end{document}
