\documentclass{ximera}
\input{../../preamble.tex}
\begin{document}


\noindent In Exercises~\ref{c13.1.1} -- \ref{c13.1.1a}, use Laplace transforms 
to compute the solution to the given initial value problem.
\begin{exercise} \label{c13.1.1}
$\ddot{x} + 3\dot{x} + 2x = 0, \quad x(0) = 1, \quad \dot{x}(0) = -1$. 

\begin{solution}
\ans The solution to the initial value problem is
$x(t) = e^{-t}$.

\soln Using properties~\eqref{Tprops}(a,c), compute:
\[
\begin{array}{rcl}
0 & = & {\cal L}[\ddot{x} + 3\dot{x} + 2x] \\
& = & (s^2{\cal L}[x] - sx(0) - \dot{x}(0)) + 3(s{\cal L}[x] - x(0))
+ 2{\cal L}[x] \\
& = & (s^2 + 3s + 2){\cal L}[x] - (3 + s)x(0) - \dot{x}(0) \\
& = & (s^2 + 3s + 2){\cal L}[x] - (s + 2).
\end{array}
\]
Simplify to obtain
\[
{\cal L}[x] = \frac{s + 2}{(s + 2)(s + 1)} = \frac{1}{s + 1}.
\]
So, using \eqref{eq:Lexp},
${\cal L}[x] = {\cal L}[e^{-t}]$.  By property \eqref{Tprops}(b),
${\cal L}^{-1}$ exists, so we can compute $x(t) = e^{-t}$.

\end{solution}
\end{exercise}
\begin{exercise} \label{c13.1.1a}
$\ddot{x} - 3\dot{x} - 4x = 0, \quad x(0) = 2, \quad \dot{x}(0) = -1$. 

\begin{solution}
\ans The solution to the initial value problem is
$\dps x(t) = -\frac{1}{5}(e^{4t}+9e^{-t})$.

\soln Using properties~\eqref{Tprops}(a,c), compute:
\[
\begin{array}{rcl}
0 & = & {\cal L}[\ddot{x} - 3\dot{x} - 4x] \\
& = & (s^2{\cal L}[x] - sx(0) - \dot{x}(0)) - 3(s{\cal L}[x] - x(0))
- 4{\cal L}[x] \\
& = & (s^2 - 3s - 4){\cal L}[x] + (3 - s)x(0) - \dot{x}(0) \\
& = & (s^2 - 3s - 4){\cal L}[x] + 7 - 2s.
\end{array}
\]
Simplify to obtain
\[
{\cal L}[x] = \frac{7-2s}{(s-4)(s+1)} = 
-\frac{1}{5}\left(\frac{1}{s-4} + \frac{9}{s+1}\right).
\]
So, using \eqref{eq:Lexp},
${\cal L}[x] = {\cal L}[-\frac{1}{5}(e^{4t}+9e^{-t})]$.  By property 
\eqref{Tprops}(b), ${\cal L}^{-1}$ exists, so we can compute 
$x(t) = -\frac{1}{5}(e^{4t}+9e^{-t})$.



\end{solution}
\end{exercise}
\end{document}
