\documentclass{ximera}
\input{../../preamble.tex}
\begin{document}

\noindent In Exercises~\ref{c12.4.1} -- \ref{c12.4.7} use the method of 
undetermined coefficients to find particular solutions to the given 
differential equations.
\begin{exercise}  \label{c12.4.1}
$(D^2-3D+2)x = \sin(t)$.

\begin{solution}
\ans One solution to the differential equation is
\[
x(t) = \frac{1}{3}\cos t + \frac{1}{6}\sin t.
\]

\soln
\paragraph{Step 1.} First, find an annihilator for $g(t) = \sin t$.  Since
$\sin t$ is a solution to any homogeneous equation with eigenvalue
$\lambda = \pm i$, the differential equation $q(D) = D^2 + 1$ is an
annihilator.

\paragraph{Step 2.} Next, find the trial space of solutions for the
differential equation.  The homogeneous equation $\ddot{x} - 3\dot{x}
+ 2 = 0$ has eigenvalues $2$ and $3$.  These eigenvalues are distinct
from $\lambda$, so the trial space is the space of solutions to $q(D)x
= 0$, which is
\[
y(t) = c_1\cos t + c_2\sin t.
\]
\paragraph{Step 3.} Now substitute $y(t)$ into the differential equation:
\[
(D^2 - 3D + 2)(y(t)) = -(c_1\sin t + c_2\cos t) + 3(c_1\sin t - c_2\cos t)
+ 2(c_1\cos t + c_2\sin t) = \sin t.
\]
Solve this system for $c_1$ and $c_2$ to find that $y(t)$ is a solution to
the differential equation when $c_1 = \frac{1}{3}$ and $c_2 = \frac{1}{6}$.

\end{solution}
\end{exercise}
\begin{exercise}  \label{c12.4.2}
$\ddot{x}+2\dot{x}+x = t + e^t$.

\begin{solution}
\ans One solution to the differential equation is
\[
x(t) = \frac{1}{4}e^t + t - 2.
\]

\soln Let $g(t) = t$ and $h(t) = e^t$.  If $p(D) = D^2 + 2D + 1$, then the
sum of solutions to $p(D)x = g(t)$ and $p(D)x = h(t)$ is a solution to
$p(D)x = g(t) + h(t)$.  First find a solution to $p(D)x = g(t)$:

\paragraph{Step 1.} Since $t$ is a solution to any homogeneous equation
with a double eigenvalue at $\lambda = 0$, the differential equation
$q_1(D) = D^2$ is an annihilator.

\paragraph{Step 2.} The homogeneous equation $p(D)x = 0$ has a double
eigenvalue at $-1$.  This eigenvalue is distinct from $\lambda$, so
the trial space is the space of solutions to $q_1(D)x = 0$, which is
\[
y(t) = c_1 + c_2t.
\]
\paragraph{Step 3.} Now substitute $y(t)$ into $p(D)x = g(t)$:
\[
(D^2 + D2 + 1)(y(t)) = 2c_2 + (c_1 + c_2)t = g(t) = t.
\]
Solve this system for $c_1$ and $c_2$ to find that $y(t)$ is a solution to
the differential equation when $c_1 = -2$ and $c_2 = 1$.

\para Now find a solution for $p(D)x = h(t)$:

\paragraph{Step 1.} In this case, since $e^t$ is a solution to any
homogeneous equation with an eigenvalue at $\mu = 1$, the differential
equation $q_2(D) = D - 1$ is an annihilator.

\paragraph{Step 2.} The eigenvalue $\mu$ is distinct from the eigenvalues
of $p(D)$, so the trial space is the space of solutions to $q_2(D)x =
0$, which is
\[
z(t) = d_1e^t.
\]
\paragraph{Step 3.} Now substitute $z(t)$ into $p(D)x = h(t)$:
\[
(D^2 + D2 + 1)(z(t)) = d_1e^t + 2d_1e^t + d_1e^t = h(t) = e^t.
\]
Solve this system for $d_1$ to find that $z(t)$ is a solution to
the differential equation when $d_1 = \frac{1}{4}$.  Now, $x(t) = y(t) + z(t)$
is a solution to the differential equation $p(D)x = t + e^t$.


\end{solution}
\end{exercise}
\begin{exercise}  \label{c12.4.3}
$(D^3+6D^2+9D+4)x = e^{-t}$.

\begin{solution}
\ans One solution to the differential equation is
\[
x(t) = \frac{1}{6}t^2e^{-t}.
\]

\soln Let $p(D) = D^3 + 6D^2 + 9D + 4$, and let $g(t) = e^{-t}$.
\paragraph{Step 1.} An annihilator for $g(t)$ is $q(D) = D + 1$, since
$g(t)$ is a solution to any homogeneous equation with an eigenvalue at
$\mu = -1$.

\paragraph{Step 2.} The equation $p(D)x = 0$ has an eigenvalue at
$\lambda_1 = -4$, and a double eigenvalue at $\lambda_2 = -1$.  Since
$\mu = \lambda_2$, we find the trial space by applying $q(D)$ to both
sides of $p(D)x = g(t)$:
\[
q(D)(D^3 + 6D^2 + 9D + 4) = D^4 + 7D^3 + 15D^2 + 13D + 4 = 0.
\]
The general solution to this differential equation is
\[
x(t) = c_1e^{-4t} + c_2e^{-t} + c_3te^{-t} + c_4t^2e^{-t}.
\]
Since any solution to the homogeneous equation is equal to zero, we can set
$c_1 = c_2 = c_3 = 0$.  So the trial space is
\[
y(t) = c_4t^2e^{-t}.
\]
\paragraph{Step 3.} Substitute $y(t)$ into $p(D)x = g(t)$:
\[
p(D)(y(t)) = \frac{d^3x}{dt^3}(c_4t^2e^{-t}) +
6\frac{d^2x}{dt^2}(c_4t^2e^{-t}) + 9\frac{dx}{dt}(c_4t^2e^{-t}) +
4(c_4t^2e^{-t}) = 6c_4e^{-t} =  e^{-t}.
\]
Solve this system for $c_4$ to find that $y(t)$ is a solution to the
differential equation when $c_4 = \frac{1}{6}$.

\end{solution}
\end{exercise}
\begin{exercise}  \label{c12.4.4}
$(D^2+D-2)x = 3te^t$.

\begin{solution}
\ans One solution to the differential equation is
\[
x(t) = \frac{3}{4}t^2e^t - \frac{1}{2}te^t.
\]
\soln Let $p(D) = D^2 + D - 2$ and let $g(t) = 3te^t$.

\paragraph{Step 1.} An annihilator for $g(t)$ is
\[
q(D) = (D - 1)^2 = D^2 - 2D + 1,
\]
since $g(t)$ is a solution to any homogeneous differential equation
with a double eigenvalue at $\mu = 1$.

\paragraph{Step 2.} The equation $p(D)x = 0$ has eigenvalues at
$\lambda_1 = -2$ and $\lambda_2 = 1$.  Since $\mu = \lambda_2$, we
find the trial space by applying $q(D)$ to both sides of $p(D)x =
g(t)$:
\[
q(D)(D^2 + D - 2) = D^4 - D^3 - 3D^2 + 5D - 2 = 0.
\]
The general solution to this differential equation is
\[
x(t) = c_1e^{-2t} + c_2e^t + c_3te^t + c_4t^2e^t.
\]
Since any solution to the homogeneous equation is equal to zero, we can set
$c_1 = c_2 = 0$.  So the trial space is
\[
y(t) = c_3te^t + c_4t^2e^t.
\]
\paragraph{Step 3.} Substitute $y(t)$ into $p(D)x = g(t)$, obtaining
\[
c_3(3e^t) + c_4(2e^t + 4te^t) = 3te^t.
\]
Solve this system for $c_3$ and $c_4$ to find that $y(t)$ is a solution
to the differential equation when $c_3 = -\frac{1}{2}$ and
$c_4 = \frac{3}{4}$.

\end{solution}
\end{exercise}
\begin{exercise}  \label{c12.4.5}
$\ddot{x}+x = t\sin t$.

\begin{solution}
\ans One solution to the differential equation is
\[
x(t) = \frac{1}{4}(t\sin t- t^2\cos t).
\]

\soln Let $p(D) = D^2 + 1$ and let $g(t) = t\sin t$.
\paragraph{Step 1.} An annihilator for $g(t)$ is
\[
q(D) = (D^2 + 1)^2 = D^4 + 2D + 1,
\]
since $g(t)$ is a solution to any homogeneous differential equation
with a double eigenvalue at $\mu = \pm i$.

\paragraph{Step 2.} The equation $p(D)x = 0$ has eigenvalue $\lambda =
\pm i$.  Since $\mu = \lambda$, we find the trial space by applying
$q(D)$ to both sides of $p(D)x = g(t)$:
\[
q(D)(D^2 + 1) = D^6 + 2D^4 + 3D^2 + 1 = 0.
\]
The general solution to this differential equation is
\[
x(t) = c_1\cos t + c_2\sin t + c_3t\cos t + c_4t\sin t + c_5t^2\cos t
+ c_6t^2\sin t.
\]
Since any solution to the homogeneous equation is equal to zero, we can
set $c_1 = c_2 = 0$.  So the trial space is
\[
y(t) = c_3t\cos t + c_4t\sin t + c_5t^2\cos t + c_6t^2\sin t.
\]
\paragraph{Step 3.} Substitute $y(t)$ into $p(D)x = g(t)$, obtaining
\[
c_3(-2\sin t) + c_4(2\cos t) + c_5(2\cos t - 4t\sin t) +
c_6(2\sin t + 4t\cos t) = t\sin t.
\]
Solve this system for the scalars $c_j$ to find that $y(t)$ is a solution
to the differential equation when $c_3 = 0$, $c_4 = \frac{1}{4}$,
$c_5 = -\frac{1}{4}$, and $c_6 = 0$.

\end{solution}
\end{exercise}
\begin{exercise}  \label{c12.4.6}
$(D^3+D)x = 6t^2+\sin t$.

\begin{solution}
\ans One solution to the differential equation is
\[
x(t) = 2t^3 - 12t - \frac{1}{2}t\sin t.
\]

\soln Let $p(D) = D^3 + D$ and let $g(t) = 6t^2$ and $h(t) = \sin t$.  Then
the sum of solutions to $p(D)x = g(t)$ and $p(D)x = h(t)$ is a solution to
$p(D)x = g(t) + h(t)$.  So, first find a solution for $p(D)x = g(t)$:
\paragraph{Step 1.} An annihilator for $g(t)$ is
\[
q_1(D) = D^3,
\]
since $g(t)$ is a solution to any homogeneous differential equation
with a triple eigenvalue at $\mu_1 = 0$.

\paragraph{Step 2.} The equation $p(D)x = 0$ has eigenvalues
$\lambda_1 = 0$ and $\lambda_2 = \pm i$.  Since $\lambda_1 = \mu_1$,
we find the trial space by applying $q_1(D)$ to both sides of $p(D)x =
g(t)$:
\[
q_1(D)(D^3 + D) = D^6 + D^4 = 0.
\]
The general solution to this differential equation is
\[
x(t) = c_1 + c_2t + c_3t^2 + c_4t^3 + c_5\cos t + c_6\sin t.
\]
Since any solution to the homogeneous equation is equal to zero, we can
set $c_1 = c_5 = c_6 = 0$.  So the trial space is
\[
y(t) = c_2t + c_3t^2 + c_4t^3.
\]
\paragraph{Step 3.} Substitute $y(t)$ into $p(D)x = g(t)$, obtaining
\[
c_2 + c_3(3t^2) + c_4(t^2 + 6) = 6t^2.
\]
Solve this system for the scalars $c_j$ to find that $y(t)$ is a solution
to $p(D)x = g(t)$ when $c_2 = -12$, $c_3 = 0$, and $c_4 = 2$.

\para Now find a solution for $p(D)x = h(t)$:

\paragraph{Step 1.} In this case, $q_2(D) = D^2 + 1$ is an annihilator,
since $h(t)$ is a solution for any homogeneous differential equation
with an eigenvalue at $\mu_2 = \pm i$.

\paragraph{Step 2.} Since $\lambda_2 = \mu_2$, we find the trial space
by applying $q_2(D)$ to both sides of $p(D)x = h(t)$:
\[
q_2(D)(D^3 + D) = D^5 + 2D^3 + D = 0.
\]
The general solution to this differential equation is
\[
x(t) = d_1 + d_2\cos t + d_3\sin t + d_4t\cos t + d_5t\sin t.
\]
Since any solution to the homogeneous equation is equal to zero, we can
set $d_1 = d_2 = d_3 = 0$.  So the trial space is
\[
z(t) = d_4t\cos t + d_5t\sin t.
\]
\paragraph{Step 3.} Substitute $z(t)$ into $p(D)x = h(t)$, obtaining
\[
d_4(-4\cos t) + d_5(-2\sin t) = \sin t.
\]
Solve this system for $d_4$ and $d_5$ to find that $z(t)$ is a solution
to $p(D)x = h(t)$ when $d_4 = 0$ and $d_5 = -\frac{1}{2}$.  So $x(t) =
y(t) + z(t)$ is a solution to $(D^3 + D)x = 6t^2 + \sin t$.

\end{solution}
\end{exercise}
\begin{exercise}  \label{c12.4.7}
$(D^2+2D+2)x = 8e^{-t}\sin t$.

\begin{solution}
\ans One solution to the differential equation is
\[
x(t) = -4te^{-t}\cos t.
\]

\soln Let $p(D) = D^2 + 2D + 2$ and let $g(t) = 8e^{-t}\sin t$.
\paragraph{Step 1.} An annihilator for $g(t)$ is
\[
q(D) = D^2 + 2D + 2,
\]
since $g(t)$ is a solution to any homogeneous differential equation
with an eigenvalue at $\mu = -1 \pm i$.

\paragraph{Step 2.} The equation $p(D)x = 0$ has eigenvalue
$\lambda = -1 \pm i$.  Since $\mu = \lambda$, we find the trial space
by applying $q(D)$ to both sides of $p(D)x = g(t)$:
\[
q(D)(D^2 + 2D + 1) = D^4 + 4D^3 + 8D^2 + 8D + 4	= 0.
\]
The general solution to this differential equation is
\[
x(t) = c_1e^{-t}\cos t + c_2e^{-t}\sin t + c_3te^{-t}\cos t +
c_4te^{-t}\sin t.
\]
Since any solution to the homogeneous equation is equal to zero, we can
set $c_1 = c_2 = 0$.  So the trial space is
\[
y(t) = c_3te^{-t}\cos t + c_4te^{-t}\sin t.
\]
\paragraph{Step 3.} Substitute $y(t)$ into $p(D)x = g(t)$, obtaining
\[
c_3(-2e^{-t}\sin t) + c_4(2e^{-t}\cos t) = 8e^{-t}\sin t.
\]
Solve this system for $c_3$ and $c_4$ to find that $y(t)$ is a solution
to the differential equation when $c_3 = -4$ and $c_4 = 0$.

\end{solution}
\end{exercise}
\end{document}
