\documentclass{ximera}
\input{../../preamble.tex}
\begin{document}
\begin{exercise}  \label{exer:at}
\begin{itemize}
\item[(a)]  Draw the direction field for
\begin{equation} \label{ex:at}
\frac{dx}{dt} = \frac{x}{x-t}.
\end{equation}
Assuming that $x(2)=3$, estimate $x(137)$.
\item[(b)]  Verify that
\[
x(t) = t + \sqrt{t^2-3}
\]
is the solution to \eqref{ex:at}.  Then show that $x(t)$ satisfies the
initial condition $x(2)=3$.
\item[(c)]  Compare your estimate of the solution to \eqref{ex:at}
obtained using {\dfield} with the exact solution
\[
x(137)= 137 +\sqrt{18766} \approx 273.989
\]
\end{itemize}

\begin{solution}

(a) The {\tt dfield5} estimate is $x(137) = 273.989$, found by zooming
in on the graph shown in Figure~\ref{exer:at}.  This figure shows the
direction field for $\frac{dx}{dt} = \frac{x}{x - t}$ with the desired
initial condition $x(2) = 3$ on the interval $0 \leq t \leq 150$, $0
\leq x \leq 300$.

(b) In order to verify that the equation $x(t) = t + \sqrt{t^2 - 3}$
is a solution to
\[
\begin{array}{rcl}
\frac{dx}{dt} & = & \frac{x}{x - t} \\
x(2) & = & 3\end{array}
\]
we must show that both of these conditions are valid for the equation.
To show that the first condition holds, take the derivative of $x(t)$.
\[
\frac{dx}{dt} = 1 + \frac{t}{\sqrt{t^2 - 3}} = \frac{t + {\sqrt{t^2 - 
3}}}{\left({\sqrt{t^2 - 3}} + t\right) - t} = \frac{x}{x - t}.
\]
To show that the second condition holds, substitute into the formula for
$x(t)$ to obtain:
\[ x(2) = 2 + \sqrt{2^2 - 3} = 3. \]

(c) The {\tt dfield5} solution coincides with the algebraic solution to at
least 3 decimal places.

\begin{figure}[htb]
                       \centerline{%
                       \psfig{file=exfigure/3-2-4.eps,width=3.0in}}
		\exercap{exer:at}
\end{figure}




\end{solution}
\end{exercise}
\end{document}
