\documentclass{ximera}
\input{../../preamble.tex}
\begin{document}
\begin{exercise} \label{c4.3.8}
The {\em cross product\/} of two $3$-vectors $x=(x_1,x_2,x_3)$
and $y=(y_1,y_2,y_3)$ is the $3$-vector
\[
x\times y = (x_2y_3-x_3y_2,-(x_1y_3-x_3y_1),x_1y_2-x_2y_1).
\]
Let $K=(2,1,-1)$.  
\begin{enumeratea}
\item Show that the mapping $L:\R^3\to\R^3$ defined by
\[
L(x) = x\times K
\]
is a linear mapping.  
\item
Find the $3\times 3$ matrix $A$ such that
\[
L(x) = Ax,
\]
that is, $L=L_A$.
\end{enumeratea}
\begin{solution}

\ans The matrix of linear mapping $L$ is
\[
A = \matthree{0}{-1}{-1}{1}{0}{2}{1}{-2}{0}.
\]

\soln Let $X = (x_1,x_2,x_3)$ and let $Y = (y_1,y_2,y_3)$.  
Since $K = (2,1,-1)$,
\[
L(X) = (x_1,x_2,x_3) \times K = 
(-x_2 - x_3, x_1 + 2x_3, x_1 - 2x_2).
\]
\begin{enumeratea}
\item To show that $L(X)$ is a linear mapping, first demonstrate that
\eqref{sum} is valid:
\[
\begin{array}{rcl}
L(X + Y) & = & L(x_1 + y_1,x_2 + y_2,x_3 + y_3) \\
& = & (-(x_2 + y_2) - (x_3 + y_3), (x_1 + y_1) + 2(x_3 + y_3),
(x_1 + y_1) - 2(x_2 + y_2)) \\
& = & (-x_2 - x_3, x_1 + 2x_3, x_1 - 2x_2) +
(-y_2 - y_3, y_1 + 2y_3, y_1 - 2y_2) \\
& = & L(X) + L(Y), \end{array}
\]
then show that \eqref{product} is valid:
\[
\begin{array}{rcl}
cL(X) & = & cL(x_1,x_2,x_3) \\
& = & c(-x_2 - x_3, x_1 + 2x_3, x_1 - 2x_2) \\
& = & (-cx_2 - cx_3, cx_1 + 2cx_3, cx_1 - 2cx_2) \\
& = & L(cx_1,cx_2,cx_3) \\
& = & L(cX). \end{array}
\]

\item Find $A$ by noting that $L(e_j) = Ae_j$ is the $j^{th}$ column of $A$,
and computing
\[ \begin{array}{l}
L(e_1) = L(1,0,0) = (0,1,1) \\
L(e_2) = L(0,1,0) = (-1,0,-2) \\
L(e_3) = L(0,0,1) = (-1,2,0). \end{array} \]
\end{enumeratea}

\end{solution}
\end{exercise}
\end{document}
