\documentclass{ximera}

\input{../preamble.tex}

\title{Nonconstant Coefficient Linear Equations}

\begin{document}
\begin{abstract}
\end{abstract}
\maketitle


\label{sec:VarConstS}

The simplest nonconstant coefficient homogeneous\index{homogeneous} 
linear differential equation is:
\begin{equation}   \label{eq:linhomo1}
\frac{dx}{dt}  =  a(t)x.
\end{equation}
This equation does not have constant coefficients, since the coefficient 
$a$ depends on $t$.  The equation is linear as linear combinations of 
solutions are solutions.  Note that \eqref{eq:linhomo1} is of the form 
\eqref{eq:ghivp} and can be solved by separation of variables. 
\index{separation of variables}

If $x(t_0)=0$, then $x(t)=0$ is the solution to the initial value problem
\eqref{eq:linhomo1}.
To solve the initial value problem $x(t_0)=x_0$ for \eqref{eq:linhomo1}
when $x_0\neq 0$, we apply the technique of separation of variables to 
this equation, which yields
\[
\ln|x| = H(t) + C,
\]
where $H(t)$ is the definite integral
\begin{equation}   \label{e:H(t)}
H(t)=\int_{t_0}^t a(\tau)d\tau.
\end{equation}
Exponentiation implies that
\[
x(t) = Ke^{H(t)}
\]
for an appropriate scalar $K$.  Indeed, if $x(t_0)=x_0$, then
\[
x_0 = x(t_0) = Ke^{H(t_0)} = Ke^0 = K.
\]
We have shown that the function 
\begin{equation} \label{E:ssv}
x(t) = x_0 e^{H(t)}
\end{equation}
is the unique solution\index{uniqueness of solutions} 
to the initial value problem\index{initial value problem} 
\eqref{eq:linhomo1} where $x(t_0)=x_0$.

\subsubsection*{An Example of a Nonconstant Coefficient Equation}

We illustrate \eqref{E:ssv} by an example. Solve the initial value problem
\[
\begin{array}{rcl}
\dps \frac{dx}{dt} & = & -\dps \frac{x}{t} \\
x(2) & = & 5.
\end{array}
\]
Since $a(t)=-\frac{1}{t}$, we can use \eqref{e:H(t)} to compute
\[
H(t)=-\int_2^t \frac{1}{\tau}d\tau = -\ln t +\ln 2 =
\ln\left(\frac{2}{t}\right).
\]
Then the solution \eqref{E:ssv} is given by
\[
x(t) = 5 e^{\ln(2/t)} = \frac{10}{t}.
\]

\subsection*{The Inhomogeneous Equation}
\index{inhomogeneous}

Next, we consider forced linear differential equations of the type
\begin{equation}   \label{eq:linode1}
\frac{dx}{dt} = a(t)x + g(t),
\end{equation}
where $a$ and $g$ are continuous functions of $t$.  The differential  
equation \eqref{eq:linode1} is homogeneous when $g=0$  and 
\index{homogeneous} inhomogeneous otherwise.  As is always the 
case, we find the general solution\index{general solution} 
to the inhomogeneous equation 
by adding the general solution to the homogeneous equation (that
we can find by separation of variables) to a particular solution to 
the inhomogeneous equation.  

\subsubsection*{Two Examples of Solutions of Inhomogeneous Equations}

(a) Find all solutions of the differential equation
\begin{equation} \label{E:ie1}
\frac{dx}{dt} = 3t^2x + 3t^2.
\end{equation}
By inspection, the constant function $x_p(t)=-1$ is a 
particular solution\index{particular solution} 
of \eqref{E:ie1}. 
Since all solutions of the homogeneous equation are of the form $Ke^{t^3}$
for some real constant $K$, it follows that the general solution of the 
inhomogeneous equation is
\[
x(t) = -1 + Ke^{t^3}.
\]

\noindent (b) Find all solutions of the differential equation
\begin{equation}  \label{E:ie2}
\frac{dx}{dt} = \left(\frac{5}{t}-t\right) x + t^6.
\end{equation}
A calculation shows that $x_p(t)=t^5$ is a particular solution of \eqref{E:ie2}. 
Since all solutions to the homogeneous equation are of the form 
$Kt^5 e^{-t^2/2}$ for some real constant $K$, it follows that the general
solution of the inhomogeneous equation is
\[
x(t) = t^5 + Kt^5 e^{-t^2/2}.
\]

\subsection*{Inhomogeneous Equations and Variation of Parameters}
\index{variation of parameters}

In Examples~\eqref{E:ie1} and \eqref{E:ie2} we guessed or were given a
particular solution\index{particular solution!variation of parameters} 
to the inhomogeneous equation.  Now we discuss 
a method for finding a particular solution to the inhomogeneous
equation \eqref{eq:linode1} when $g(t)$ is a nonzero function.   This 
technique for finding a particular solution is called 
{\em variation of parameters\/}.  

We already know by separation of variables that every solution of the 
{\em homogeneous\/} equation ($g=0$) has the form $Ke^{H(t)}$ where 
$\frac{dH}{dt}=a$.  The idea behind variation of parameters is to
allow $K$ to depend on $t$.    \index{variation of parameters}
More precisely, assume that a solution $x(t)$ has the form
\[
x(t) = c(t)e^{H(t)},
\]
where $c$ is a differentiable function of $t$.  Substituting $x(t)$ in 
\eqref{eq:linode1}, using the product rule for differentiation and suppressing
the explicit dependence of functions on $t$, leads to the identity
\[
\frac{dc}{dt}e^{H}+ce^{H}a =  ace^{H}+g,
\]
which simplifies to
\[
\frac{dc}{dt} = ge^{-H}.
\]
This last equation may be solved for $c(t)$ by integration, obtaining
\begin{equation}   \label{eq:c(t)}
c(t) = \int g(\tau)e^{-H(\tau)}d\tau.
\end{equation}
Uniqueness of solutions\index{uniqueness of solutions} to initial 
value problems implies the main result of this section.

\begin{theorem}[Variation of Parameters]  \label{thm:varpar}
\index{variation of parameters}
The unique solution to the initial value problem
\index{variation of parameters!initial value problem}
\[
\begin{array}{rcl}
\dps \frac{dx}{dt} & = & a(t)x+g(t) \\
x(t_0) & = & x_0.
\end{array}
\]
is
\[
x(t) = c(t)e^{H(t)},
\]
where 
\[
H(t)=\int_{t_0}^t a(\tau)d\tau \AND
c(t)=\int_{t_0}^t g(\tau)e^{-H(\tau)}d\tau + x_0.
\]
\end{theorem} \index{variation of parameters}


\subsubsection*{Two Examples of Variation of Parameters}

(a)   Solve the initial value problem
\begin{equation} \label{e:solntheq}
\begin{array}{rcl}
\dps \frac{dx}{dt} & = & -\dps \frac{x}{t} + \frac{2}{t^4}\\
x(1) & = & 0.
\end{array}
\end{equation}
Compute
\[
H(t)= -\int_1^t\frac{1}{\tau}d\tau = -\ln t +\ln 1 = -\ln t.
\]
Hence 
\[
c(t)=\int_1^t \frac{2}{\tau^4}e^{\ln\tau}d\tau + 0
=\int_1^t \frac{2}{\tau^3} d\tau = -\frac{1}{t^2}+1
\]
which implies that 
\begin{equation}  \label{e:solnth}
x(t)=\left(1-\frac{1}{t^2}\right)\frac{1}{t}
\end{equation}
is the solution. For comparison we show the graph of \eqref{e:solnth} in 
Figure~\ref{F:solnmd}(left) and the result of a numerical computation of 
the initial value problem using {\dfield}\index{\computer!dfield8} 
in Figure~\ref{F:solnmd}(right).

\begin{figure*}[htb]
           \centerline{%
           \psfig{file=../figures/solnm.eps,width=2.8in}
           \psfig{file=../figures/solnd.eps,width=3.0in}}
           \caption{(Left) Graph of solution~\protect\eqref{e:solnth} to equation 
	\protect\eqref{e:solntheq}. (Right) The time series for solution to 
	\protect\eqref{e:solntheq} with initial condition $x(1)=0$ using 
	{\dfield}.}
           \label{F:solnmd}
\end{figure*}

\noindent (b) Solve the initial value problem
\[
\begin{array}{rcl}
\dps \frac{dx}{dt} & = & 4x + \cos t + e^{2t} \\
x(0) & = & 1.
\end{array}
\]
Here $H(t)=4t$ and 
\begin{eqnarray*}
c(t) & = &  \int_0^t g(\tau)e^{-4\tau} d\tau +1\\
& = & \int_0^t \left(\cos\tau + e^{2\tau}\right)e^{-4\tau} d\tau
+1\\
& = & \frac{1}{17}\left( e^{-4t}(\sin t - 4\cos t)+4\right) +
\frac{1}{2}\left(1-e^{-2t}\right) + 1.
\end{eqnarray*}
Thus, the solution is
\[
x(t)=c(t) e^{4t} = \frac{1}{17}(\sin t - 4\cos t+4e^{4t}) -
\frac{1}{2}e^{2t} + \frac{3}{2}e^{4t}.
\]


\EXER

\TEXER 

\noindent In Exercises~\ref{c14.2.1a} -- \ref{c14.2.1f} decide whether 
or not the given differential equation is linear.  If it is linear, 
specify whether the equation is homogeneous or inhomogeneous.
\begin{exercise}  \label{c14.2.1a}
$\dps \frac{dx}{dt} = 0$.

\begin{solution}
The differential equation is linear and homogeneous.

\end{solution}
\end{exercise}
\begin{exercise}  \label{c14.2.1b}
$\dps \frac{dx}{dt} = x^2\cos t$.

\begin{solution}
The differential equation is nonlinear.

\end{solution}
\end{exercise}
\begin{exercise}  \label{c14.2.1c}
$\dps \frac{dx}{dt} = x+t^2$.

\begin{solution}
The differential equation is linear and inhomogeneous.

\end{solution}
\end{exercise}
\begin{exercise}  \label{c14.2.1d}
$\dps \frac{dx}{dt} = \frac{t}{x}-\frac{1}{t}$.

\begin{solution}
The differential equation is nonlinear.

\end{solution}
\end{exercise}
\begin{exercise}  \label{c14.2.1e}
$\dps (t^2+1)\frac{dx}{dt} = x+\sin t$.

\begin{solution}
The differential equation is linear and inhomogeneous.

\end{solution}
\end{exercise}
\begin{exercise} \label{c14.2.1f}
$\dps x\frac{dx}{dt} = \cos t$

\begin{solution}
The differential equation is nonlinear.

\end{solution}
\end{exercise}

\noindent In Exercises~\ref{c14.2.6a} -- \ref{c14.2.6d} solve the given 
initial value problems by variation of parameters.
\begin{exercise}   \label{c14.2.6a}
$\dps \frac{dx}{dt} = t^2 x + t^2, \quad x(1)=1$.

\begin{solution}
\ans The solution to the initial value problem is
$x(t) = 2e^{\frac{1}{3}(t^3 - 1)} - 1$.

\soln By inspection $x(t) = -1$ is a solution to the inhomogeneous
equation.  The solution to the homogeneous equation $\dot{x}(t) = t^2x$ is
$x(t) = Ke^{H(t)}$, where
\[
H(t) = \int t^2dt = \frac{1}{3}t^3.
\]
So the general solution to the inhomogeneous equation is
\[
x(t) = Ke^{\frac{1}{3}t^3} - 1.
\]
Substitute the initial condition $x(1) = 1$ into this equation and
solve for $K = 2e^{-\frac{1}{3}}$.


\end{solution}
\end{exercise}
\begin{exercise}   \label{c14.2.6b}
$\dps \frac{dx}{dt} = x+2t, \quad x(0)=-1$.

\begin{solution}
\ans The solution to the initial value problem is
$x(t) = e^t - 2t - 2$.

\soln The solution to the homogeneous equation $\dot{x}=x$ is $x(t)=ce^t$
for some constant $c$.  The method of variation of parameters looks for 
solutions to the inhomogeneous equation of the form $x(t)=c(t)e^t$.  If this 
$x(t)$ is a solution to the inhomogeneous equation $\dot{x}=x+2t$, then
\[
x+2t=\dot{x}=\dot{c}e^t+ce^t = \dot{c}e^t+x.
\]
Therefore,
\[
\dot{c} = 2te^{-t}.
\]
Integrating by parts yields
\[
c(t) = 2\int te^{-t}dt = -2(t+1)e^{-t} + K.
\]
Thus the general solution to the inhomogeneous equation is:
\[
x(t) = -2(t+1) + Ke^t.
\]
Using the initial condition $x(0)=-1$ yields $K=1$. 

\end{solution}
\end{exercise}
\begin{exercise}   \label{c14.2.6c}
$\dps \frac{dx}{dt} = 
\frac{t}{t^2+1}x+\sin(t)\sqrt{t^2+1},\quad x(0)=2$.

\begin{solution}
\ans The solution to the initial value problem is
$x(t) = (3 - \cos t)\sqrt{t^2 + 1}$.

\soln By Theorem~\ref{thm:varpar}, the
solution to the initial value problem is $x(t) = c(t)e^{H(t)}$, where
$\frac{dx}{dt} = a(t)x + g(t)$.  So
\[
H(t) = \int_{t_0}^t a(\tau)d\tau = \int_0^t\frac{\tau}{\tau^2 + 1}d\tau
= \ln\sqrt{t^2 + 1}.
\]
\[
c(t) = \int_{t_0}^t g(\tau)e^{-H(\tau)}d\tau + x_0
= \int_0^t \sin(\tau)d\tau + 2
= 3 - \cos t.
\]

\end{solution}
\end{exercise}
\begin{exercise}   \label{c14.2.6d}
$\dps \frac{dx}{dt} = 2x+\frac{1}{t}e^{2t}, \quad x(1)=4$.

\begin{solution}
\ans The solution to the initial value problem is
\[
x(t) = e^{2t}(4e^{-2}+\ln t).
\]

\soln The solution to the homogeneous equation $\dot{x}=2x$ is $x(t)=e^{2t}$.
 Using variation of parameters we look for a solution to the inhomogeneous
equation $\dot{x}=2x+\frac{1}{t}e^{2t}$ of the form $x(t)=c(t)e^{2t}$.  If
$x(t)$ is a solution to the inhomogeneous equation, then
\[
2x+\frac{1}{t}e^{2t} =\dot{x}=\dot{c}e^{2t}+2ce^{2t} = \dot{c}e^{2t}+2x.
\]
Therefore, 
\[
\dot{c} = \frac{1}{t},
\]
and 
\[
c(t) = \ln|t| + K.
\]
The general solution to the inhomogeneous equation is:
\[
x(t) = (\ln|t| + K)e^{2t}.
\]
Using the initial condition $x(1)=4$, we find that $K=4e^{-2}$.



\end{solution}
\end{exercise}



\CEXER

\noindent In Exercises~\ref{c14.2.11a} -- \ref{c14.2.11c} use 
{\dfield}\index{\computer!dfield8} 
to compute solutions to the given linear differential equations.  What is 
the asymptotic behavior of the solutions as $t$ tends to infinity?  Use 
variation of parameters to explain the behavior.
\begin{exercise}   \label{c14.2.11a}
$\dps\frac{dx}{dt} = -2 x + t$.

\begin{solution}
Using {\sf dfield5} we see in Figure~\ref{c14.2.11a} that
solutions are asymptotic to a line parallel to $x=\frac{1}{2}t$.

\begin{figure}[htb]
     \centerline{%
     \psfig{file=exfigure/fig17-1-11.eps,width=3.0in}}
        \exercap{c14.2.11a}
\end{figure} 
Using variation of parameters we find that the general solution to the
differential equation $\dot{x}=-2x+t$ is 
\[
x(t) = \frac{1}{2}\left(t-\frac{1}{2}\right) +Ke^{-2t}.
\]
As $t\to\infty$, the solution $x(t)$ approaches the straight line 
$x= \frac{1}{2}t-\frac{1}{4}$.

\end{solution}
\end{exercise}
\begin{exercise}   \label{c14.2.11b}
$\dps\frac{dx}{dt} = -2 x + t^2$.

\begin{solution}
Using {\sf dfield5} and variation of parameters we see in 
Figure~\ref{c14.2.11b} that solutions are asymptotic to the
parabola $x=\frac{1}{2}((t-frac{1}{2})^2+\frac{1}{4})$.
Using variation of parameters we find that the general solution to the
differential equation $\dot{x}=-2x+t^2$ is 
\[
x(t) = \frac{1}{2}\left(t^2-t+\frac{1}{2}\right) + Ke^{-2t}.
\]
As $t\to\infty$, the solution $x(t)$ approaches the parabola  
$x= \frac{1}{2}(t^2-t+\frac{1}{2})$ --- which is verified by the 
{\sf dfield5} calculations shown in Figure~\ref{c14.2.11b}.

\begin{figure}[htb]
     \centerline{%
     \psfig{file=exfigure/fig17-1-12.eps,width=3.0in}}
        \exercap{c14.2.11b}
\end{figure} 

\end{solution}
\end{exercise}
\begin{exercise}   \label{c14.2.11c}
$\dps\frac{dx}{dt} = -2 x + \sin t$.

\begin{solution}

Using {\sf dfield5} and variation of parameters we see in 
Figure~\ref{c14.2.11c} that solutions are asymptotic to the
periodic function $x=\frac{1}{5}(\cos t-2\sin t)$.
Using variation of parameters we find that the general solution to the
differential equation $\dot{x}=-2x+\sin t$ is 
\[
x(t) = \frac{1}{5}(\cos t-2\sin t) + Ke^{-2t}.
\]
As $t\to\infty$, the solution $x(t)$ approaches the function  
$x= \frac{1}{5}(\cos t-2\sin t)$ --- which is verified by the 
{\sf dfield5} calculations shown in Figure~\ref{c14.2.11c}.

\begin{figure}[htb]
     \centerline{%
     \psfig{file=exfigure/fig17-1-13.eps,width=3.0in}}
        \exercap{c14.2.11c}
\end{figure} 



\end{solution}
\end{exercise}




\end{document}
