\documentclass{ximera}
\input{../../preamble.tex}
\begin{document}

\noindent In Exercises~\ref{c14.1.5a} -- \ref{c14.1.5c} solve the given 
initial value problem by separation of variables. 
\begin{exercise}  \label{c14.1.5a}
$\dps \frac{dx}{dt} = -3x,\quad x(0)=-1.$

\begin{solution}
\ans The solution to the given initial value problem is
\[
x(t) = -e^{-3t}.
\]
\soln Use separation of variables., as follows.  rewrite the differential 
equation as
\[
\frac{1}{x}\frac{dx}{dt} = -3.
\]
Integrate both sides, obtaining 
\[
\ln|x| = -3t + C.
\]
Determine $C$ using the initial condition $(t_0,x_0)=(0,-1)$, obtaining
$C=0$.  Exponentiate to obtain 
\[
|x(t)| = e^{-3t}
\]
and use the initial condition to determine the correct sign.

\end{solution}
\end{exercise}
\begin{exercise}  \label{c14.1.5b}
$\dps \frac{dx}{dt} = \frac{t^3-1}{\cos x},
\quad x(\pi)=\frac{\pi}{2}.$

\begin{solution}
\ans The solution to the given initial value problem is
\[
x(t) = \sin^{-1}\left(\frac{1}{4}(t^4 - 4t - \pi^4 + 4\pi + 4)\right).
\]
\soln Rewrite the differential equation as
\[
\cos(x) \frac{dx}{dt} = t^3 - 1
\]
and integrate both sides to obtain
\[
\sin x = \frac{1}{4}t^4 - t + C,
\]
for some constant $C$.  Determine $C$ using the initial condition 
$(t_0,x_0)=(\pi,\pi/2)$, that is,
\[
C = \sin\left(\frac{\pi}{2}\right) - \frac{1}{4}\pi^4 + \pi 
= 1 - \frac{1}{4}\pi^4 + \pi.
\]
Therefore,
\[
\sin x = \frac{1}{4}t^4 - t + 1 - \frac{1}{4}\pi^4 + \pi.
\]
Solve for $x$ to obtain the closed form solution to the initial value problem.


\end{solution}
\end{exercise}
\begin{exercise}  \label{c14.1.5c}
$\dps \frac{dx}{dt} = 2\sqrt{tx},\quad x(1)=1.$

\begin{solution}
\ans The solution to the given initial value problem is
\[
x(t) = \frac{1}{9}(2t^{3/2} + 1)^2.
\]
\soln Rewrite the differential equation as 
\[
\frac{1}{2\sqrt{x}}\frac{dx}{dt} = \sqrt{t}.
\]
Integrate both sides to obtain
\[
\sqrt{x} = \frac{2}{3}t^{3/2} + C.
\]
Determine $C$ using the initial condition $(t_0,x_0)=(1,1)$, that is,
\[
C = \sqrt{1} - \frac{2}{3}1^{3/2} = \frac{1}{3}.
\]
Therefore
\[
\sqrt{x} = \frac{1}{3}(2t^{3/2} + 1).
\]
Solve for $x$ to obtain the closed form solution to the initial value problem.

\end{solution}
\end{exercise}
\end{document}
