\documentclass{ximera}
\input{../../preamble.tex}
\begin{document}

\noindent In Exercises~\ref{c14.1.8a} -- \ref{c14.1.8c} use separation 
of variables to find all the solutions of the given differential equation.
\begin{exercise}  \label{c14.1.8a}
$\dps \frac{dx}{dt} = 2x$.

\begin{solution}
\ans The general solution to the differential equation is
$x(t) = Ke^{2t}$ for some $K \geq 0$.  Note that when $K = 0$, $x(t) = 0$ is
a constant solution.


\soln The differential equation can be written $\frac{dx}{dt} = g(x)h(t)$,
where $g(x) = 2x$ and $h(t) = 1$.  Then $x(t)$ satisfies
\[
G(x(t)) = H(t) + C.
\]
For nonzero $x(t)$,
\[
G(x) = \int\frac{1}{g(x)}dx = \int\frac{1}{2x}dx = \frac{1}{2}\ln|x|
\AND
H(x) = \int dt = t.
\]
So, $x(t)$ satisfies
\[
\frac{1}{2}\ln|x| = t + C.
\]
Solve for $x(t)$ to obtain the solution to the differential equation.


\end{solution}
\end{exercise}
\begin{exercise}  \label{c14.1.8b}
$\dps \frac{dx}{dt} = 5x+2$.

\begin{solution}
\ans The general solution to the differential equation is 
\[
x(t) = Ke^{5t} - \frac{2}{5}
\]
for some $K \geq 0$.  Note that $x(t) = x_0 = -\frac{2}{5}$ is a constant
solution.

\soln The differential equation can be written $\frac{dx}{dt} = g(x)h(t)$,
where $g(x) = 5x + 2$ and $h(t) = 1$.  Then $x(t)$ satisfies
\[
G(x(t)) = H(t) + C.
\]
For $x(t) \neq -\frac{2}{5}$,
\[
G(x) = \int\frac{1}{g(x)}dx = \int\frac{1}{5x + 2}dx = \frac{1}{5}\ln|5x + 2|
\AND
H(x) = \int dt = t.
\]
So, $x(t)$ satisfies
\[
\frac{1}{5}\ln|5x + 2| = t + C.
\]
Solve for $x(t)$ to obtain the solution to the differential equation.


\end{solution}
\end{exercise}
\begin{exercise}  \label{c14.1.8c}
$\dps \frac{dx}{dt} = \frac{\sin t}{x}$.

\begin{solution}
\ans The general solution to the differential equation is
$x(t) = \sqrt{2(C - \cos t)}$.

\soln The differential equation can be written $\frac{dx}{dt} = g(x)h(t)$,
where $g(x) = \frac{1}{x}$ and $h(t) = \sin t$.  Then $x(t)$ satisfies
\[
G(x(t)) = H(t) + C,
\]
where
\[
G(x) = \int\frac{1}{g(x)}dx = \int xdx = \frac{x^2}{2}
\AND
H(x) = \int h(t)dt = \int(\sin t)dt = -\cos t.
\]
So, $x(t)$ satisfies
\[
\frac{x^2}{2} = -\cos t + C.
\]
Solve for $x(t)$ to obtain the solution to the differential equation.

\end{solution}
\end{exercise}
\end{document}
