\documentclass{ximera}

\input{../preamble.tex}

\title{Composition and Multiplication of Matrices}

\begin{document}
\begin{abstract}
\end{abstract}
\maketitle

 \label{S:4.6}
\index{composition} \index{matrix!multiplication}

The {\em composition\/} of two matrix mappings leads to another
matrix mapping from which the concept of multiplication of two
matrices follows.  Matrix multiplication can be introduced by
formula, but then the idea is unmotivated and one is left to
wonder why matrix multiplication is defined in such a seemingly
awkward way.

We begin with the example of $2\times 2$ matrices.  Suppose that
\[
A= \left(\begin{array}{rr} 2 & 1\\ 1 & -1\end{array}\right)
\AND
B= \left(\begin{array}{rr} 0 & 3\\ -1 & 4\end{array}\right).
\]
We have seen that the mappings
\[
x\mapsto Ax \AND x\mapsto Bx
\]
map $2$-vectors to $2$-vectors.  So we can ask what happens when
we compose these mappings.  In symbols, we compute
\[
L_A\compose L_B (x) = L_A(L_B(x))= A(Bx).
\]
In coordinates, let $x=(x_1, x_2)$ and compute
\begin{eqnarray*}
A(Bx) & = & A \left(\begin{array}{c} 3x_2 \\ -x_1+4x_2
\end{array}\right)\\
 & = & \left(\begin{array}{c} -x_1+10x_2  \\ x_1-x_2
\end{array}\right).
\end{eqnarray*}
It follows that we can rewrite $A(Bx)$ using multiplication of a
matrix times a vector as
\[
A(Bx) = \left(\begin{array}{rr} -1 & 10 \\ 1 & -1
\end{array}\right)
        \left(\begin{array}{c} x_1 \\ x_2 \end{array} \right).
\]
In particular, $L_A\compose L_B$ is again a linear mapping,
namely $L_C$, where
\[
C =\left(\begin{array}{rr} -1 & 10 \\ 1 & -1 \end{array}\right).
\]
With this computation in mind, we define the product
\[
AB =
\left(\begin{array}{rr} 2 & 1\\ 1 & -1\end{array}\right)
\left(\begin{array}{rr} 0 & 3\\ -1 & 4\end{array}\right)
= \left(\begin{array}{rr} -1 & 10 \\ 1 & -1 \end{array}\right).
\]

Using the same approach we can derive a formula for matrix
multiplication of $2\times 2$ matrices.  Suppose
\[
A= \left(\begin{array}{rr} a_{11} & a_{12}\\ a_{21} &
a_{22}\end{array}\right)
\AND
B= \left(\begin{array}{rr} b_{11} & b_{12}\\ b_{21} &
b_{22}\end{array}\right).
\]
Then
\begin{eqnarray*}
A(Bx) & = & A \left(\begin{array}{c} b_{11}x_1+b_{12}x_2 \\
b_{21}x_1+b_{22}x_2 \end{array}\right)\\
 & = & \left(\begin{array}{c} a_{11}(b_{11}x_1+b_{12}x_2)
+a_{12}(b_{21}x_1+b_{22}x_2)  \\
a_{21}(b_{11}x_1+b_{12}x_2) +
a_{22}(b_{21}x_1+b_{22}x_2) \end{array}\right) \\
 & = & \left(\begin{array}{c} (a_{11}b_{11}+a_{12}b_{21})x_1+
(a_{11}b_{12}+a_{12}b_{22})x_2  \\
(a_{21}b_{11}+a_{22}b_{21})x_1+
(a_{21}b_{12}+a_{22}b_{22})x_2 \end{array}\right) \\
& = & \left(\begin{array}{rr} a_{11}b_{11}+a_{12}b_{21} &
a_{11}b_{12}+a_{12}b_{22}\\
a_{21}b_{11}+a_{22}b_{21} & a_{21}b_{12}+a_{22}b_{22}
\end{array}\right)
        \left(\begin{array}{c} x_1 \\ x_2 \end{array} \right).
\end{eqnarray*}
Hence, for $2\times 2$ matrices, we see that composition of
matrix mappings defines the matrix multiplication\index{matrix!multiplication}
\begin{equation*}
\left(\begin{array}{rr} a_{11} & a_{12}\\ a_{21} &
a_{22}\end{array}\right)
\left(\begin{array}{rr} b_{11} & b_{12}\\ b_{21} &
b_{22}\end{array}\right)
\end{equation*}
to be
\begin{equation}  \label{2x2mult}
\left(\begin{array}{rr} a_{11}b_{11}+a_{12}b_{21} &
a_{11}b_{12}+a_{12}b_{22}
\\ a_{21}b_{11}+a_{22}b_{21} & a_{21}b_{12}+a_{22}b_{22}
\end{array}\right).
\end{equation}

Formula \eqref{2x2mult} may seem a bit formidable, but it does
have structure.  Suppose $A$ and $B$ are $2\times 2$ matrices,
then the entry of
\[
C=AB
\]
in the $i^{th}$ row, $j^{th}$ column may be written as
\[
a_{i1}b_{1j} + a_{i2}b_{2j} = \sum_{k=1}^2 a_{ik}b_{kj}.
\]
We shall see that an analog of this formula is available for
matrix multiplications of all sizes.  But to derive this
formula, it is easier to develop matrix multiplication
abstractly.


\begin{lemma}  \label{complin}
Let $L_1:\R^n\to\R^m$ and $L_2:\R^p\to\R^n$ be linear mappings.
Then $L=L_1\compose L_2:\R^p\to\R^m$ is a linear mapping.
\end{lemma}

\begin{proof}  Compute
\begin{eqnarray*}
L(x+y) & = & L_1\compose L_2(x+y)\\
 & = & L_1(L_2(x)+L_2(y)) \\
 & = & L_1(L_2(x)) + L_1(L_2(y))\\
 & = & L_1\compose L_2(x) + L_1\compose L_2(y)\\
 & = & L(x) + L(y).
\end{eqnarray*}
Similarly, compute $L_1\compose L_2(cx) = cL_1\compose L_2(x)$.
\end{proof}

We apply Lemma~\ref{complin} in the following way.  Let $A$ be
an $m\times n$ matrix and let $B$ be an $n\times p$
matrix.  Then $L_A:\R^n\to\R^m$ and $L_B:\R^p\to\R^n$ are linear
mappings, and the mapping $L=L_A\compose L_B:\R^p\to\R^m$ is
defined and linear.  Theorem~\ref{lin-matrices} implies that
there is an $m\times p$ matrix $C$ such that $L=L_C$.
Abstractly, we define the {\em matrix product\/} \index{matrix!product}
$AB$ to be $C$.
\begin{quote}
{\em Note that the matrix product $AB$ is defined only when the number of
columns of $A$ is equal to the number of rows of $B$.}
\end{quote}

\subsubsection*{Calculating the Product of Two Matrices}

Next we discuss how to calculate the product of matrices; this
discussion generalizes our discussion of the product of $2\times 2$
matrices.  Lemma~\ref{columnsA} tells how to compute $C=AB$.  The $j^{th}$
column of the matrix product is just
\[
Ce_j = A(Be_j),
\]
where $B_j\equiv Be_j$ is the $j^{th}$ column of the matrix $B$.  Therefore,
\begin{equation}  \label{E:matprod}
C = (AB_1|\cdots|AB_p).
\end{equation}
Indeed, the $(i,j)^{th}$ entry of $C$ is the $i^{th}$ entry of $AB_j$,
that is, the $i^{th}$ entry of
\[
A\left(\begin{array}{c} b_{1j}\\ \vdots\\
b_{nj}\end{array}\right)
=
\left(\begin{array}{c} a_{11}b_{1j} + \cdots + a_{1n}b_{nj} \\
\vdots \\ a_{m1}b_{1j} + \cdots + a_{mn}b_{nj}
\end{array}\right).
\]
It follows that the entry $c_{ij}$ of $C$ in the $i^{th}$ row and
$j^{th}$ column is
\begin{equation} \label{multij}
c_{ij} = a_{i1}b_{1j} + a_{i2}b_{2j} + \cdots + a_{in}b_{nj} =
\sum_{k=1}^n a_{ik}b_{kj}.
\end{equation}

We can interpret \eqref{multij} in the following way.  To calculate $c_{ij}$:
multiply the entries of the $i^{th}$ row of $A$ with the corresponding
entries in the $j^{th}$ column of $B$ and add the results.  This
interpretation reinforces the
idea that for the matrix product $AB$ to be defined, the number of columns
in $A$ must equal the number of rows in $B$.

For example, we now perform the following multiplication:

\begin{eqnarray*}
& & \left(\begin{array}{rrr} 2 & 3 & 1 \\ 3 & -1 & 2 \end{array}\right)
\left(\begin{array}{rr} 1 & -2 \\ 3 & 1 \\ -1 & 4 \end{array}\right)\\
& = & \mattwoc{2\cdot 1+3\cdot 3 + 1\cdot(-1)}{2\cdot(-2)+3\cdot 1+1\cdot 4}
{3\cdot 1 + (-1)\cdot 3+2\cdot(-1)}{3\cdot(-2)+(-1)\cdot 1+2\cdot 4}\\
& = & \mattwo{10}{3}{-2}{1}.
\end{eqnarray*}

\subsubsection*{Some Special Matrix Products}

Let $A$ be an $m\times n$ matrix.  Then
\begin{eqnarray*}
OA & = & O \\
AO & = & O \\
AI_n & = & A \\
I_mA & = & A
\end{eqnarray*}
The first two equalities are easily checked using \eqref{multij}.
It is not significantly more difficult to verify the last two
equalities using \eqref{multij}, but we shall verify these
equalities using the language of linear mappings, as follows:
\[
L_{AI_n}(x)=L_A\compose L_{I_n}(x)=L_A(x),
\]
since $L_{I_n}(x)=x$ is the identity map.  Therefore $AI_n=A$.
A similar proof verifies that $I_mA=A$.  Although the
verification of these equalities using the notions of linear
mappings may appear to be a case of overkill, the next section
contains results where these notions truly simplify the discussion.

\EXER

\TEXER

\noindent In Exercises~\ref{c4.6.-1a} -- \ref{c4.6.-1d} determine whether or 
not the matrix products $AB$ or $BA$ can be computed for each given pair of 
matrices $A$ and $B$.  If the product is possible, perform the computation.
\begin{exercise}  \label{c4.6.-1a}
$A=\mattwo{1}{0}{-2}{1}$ and $B=\mattwo{-2}{0}{3}{-1}$.

\begin{solution}
$AB=\mattwo{-2}{0}{7}{-1}$ and $BA= \mattwo{-2}{0}{5}{-1}$.

\end{solution}
\end{exercise}
\begin{exercise}  \label{c4.6.-1b}
$A=\left(\begin{array}{rrr} 0 & -2 & 1\\ 4 & 10 & 0 \end{array}\right)$
and $B=\left(\begin{array}{rr} 0 & 2 \\ 3 & -1 \end{array}\right)$.

\begin{solution}
$AB$ is not defined. $BA=\left(\begin{array}{rrr} 8 &  20 &  0\\
 -4 & -16  &  3\end{array}\right)$


\end{solution}
\end{exercise}
\begin{exercise}  \label{c4.6.-1c}
$A=\left(\begin{array}{rrrr} 8 & 0 & 2 & 3\\ -3 & 0 & -10 &
3\end{array}\right)$
and $B=\left(\begin{array}{rrr} 0 & 2 & 5\\ -1 & 3 & -1 \\ 0 & 1 &
-5\end{array}\right)$.

\begin{solution}
$AB$ is not defined. $BA$  is not defined.  

\end{solution}
\end{exercise}
\begin{exercise}  \label{c4.6.-1d}
$A=\left(\begin{array}{rr} 8 & -1 \\ -3 & 12 \\ 5 & -4\end{array}\right)$
and $B=\left(\begin{array}{rrrr} 2 & 8 & 0 & -3\\ 1 & 4 & 0 & 1\\
-5 & 6 & 7 & -20\end{array}\right)$

\begin{solution}
$AB$ is not defined. $BA$  is not defined.


\end{solution}
\end{exercise}

\noindent In Exercises~\ref{c4.6.0a} -- \ref{c4.6.0d} compute
the given matrix product.
\begin{exercise}  \label{c4.6.0a}
$\mattwo{2}{3}{0}{1}\mattwo{-1}{1}{-3}{2}$.

\begin{solution}

$\mattwo{2}{3}{0}{1}\mattwo{-1}{1}{-3}{2} =
\cmattwo{-2 - 9}{2+6}{-3}{2} = \mattwo{-11}{8}{-3}{2}$.

\end{solution}
\end{exercise}
\begin{exercise}  \label{c4.6.0b}
$\left(\begin{array}{rrr} 1 & 2 & 3\\ -2 & 3 & -1 \end{array}\right)
\left(\begin{array}{rr} 2 & 3\\ -2 & 5 \\1 & -1 \end{array}\right)$.

\begin{solution}

$\left(\begin{array}{rrr} 1 & 2 & 3\\ -2 & 3 & -1 \end{array}\right)
\left(\begin{array}{rr} 2 & 3\\ -2 & 5 \\1 & -1 \end{array}\right)
= \mattwo{2 - 4 + 3}{3 + 10 - 3}{-4 - 6 - 1}{-6 + 15 + 1}
= \mattwo{1}{10}{-11}{10}$.

\end{solution}
\end{exercise}
\begin{exercise}  \label{c4.6.0c}
$\left(\begin{array}{rr} 2 & 3\\ -2 & 5 \\1 & -1 \end{array}\right)
\left(\begin{array}{rrr} 1 & 2 & 3\\ -2 & 3 & -1 \end{array}\right)$.

\begin{solution}
$\left(\begin{array}{rr} 2 & 3\\ -2 & 5 \\1 & -1 \end{array}
\right) \left(\begin{array}{rrr} 1 & 2 & 3\\ -2 & 3 & -1 \end{array}\right)
= \matthree{-4}{13}{3}{-12}{11}{-11}{3}{-1}{4}$.

\end{solution}
\end{exercise}
\begin{exercise}  \label{c4.6.0d}
$\left(\begin{array}{rrr} 2 & -1 &3\\ 1 & 0 & 5\\1 & 5 & -1\end{array}\right)
\left(\begin{array}{rrr} 1 & 7 \\ -2 & -1 \\ -5 & 3\end{array}\right)$.

\begin{solution}

$\left(\begin{array}{rrr} 2 &  -1 &3\\ 1 & 0 & 5 \\1 & 5 & -1
\end{array}\right)
\left(\begin{array}{rrr} 1 & 7 \\ -2 & -1 \\ -5 & 3\end{array}\right)
= \left(\begin{array}{cc} 2+2-15 & 14+1+9 \\ 1-25 & 7+15 \\
1-10+5 & 7-5-3 \end{array}\right)
= \left(\begin{array}{rr} -11 & 24 \\ -24 & 22 \\ -4 & -1
\end{array}\right)$.


\end{solution}
\end{exercise}


\begin{exercise} \label{c4.6.1}
Determine all the $2\times 2$ matrices $B$ such that $AB=BA$
where $A$ is the matrix
\[
A=\left(\begin{array}{rr} 2 & 0 \\ 0 & -1 \end{array}\right).
\]

\begin{solution}

\ans For any matrix $B$ of the form
\[
\mattwo{b_{11}}{0}{0}{b_{22}}
\]
the equation $AB = BA$ is valid.

\soln Let
\[
B = \mattwo{b_{11}}{b_{12}}{b_{21}}{b_{22}}.
\]
Then compute the matrix $B$ for which
\[
\begin{array}{rcl}
AB & = & BA \\
\mattwo{2}{0}{0}{-1}\mattwo{b_{11}}{b_{12}}{b_{21}}{b_{22}} &
= & \mattwo{b_{11}}{b_{12}}{b_{21}}{b_{22}}\mattwo{2}{0}{0}{-1} \\
\mattwo{2b_{11}}{2b_{12}}{-b_{21}}{-b_{22}} & = &
\mattwo{2b_{11}}{-b_{12}}{2b_{21}}{-b_{22}} \end{array}
\]
which is equivalent to the linear system
\[
\begin{array}{l}
2b_{11} = 2b_{11} \\
2b_{12} = -b_{12} \\
-b_{21} = 2b_{21} \\
-b_{22} = -b_{22}. \end{array}
\]

\end{solution}
\end{exercise}

\begin{exercise} \label{c4.6.2}
Let
\[
A=\mattwo{2}{5}{1}{4} \AND B=\mattwo{a}{3}{b}{2}.
\]
For which values of $a$ and $b$ does $AB=BA$?

\begin{solution}

\ans 
\[
B = \mattwo{\frac{4}{5}}{3}{\frac{3}{5}}{2}.
\]

\soln Compute
\[
\begin{array}{rcl}
AB & = & BA \\
\mattwo{2}{5}{1}{4}\mattwo{a}{3}{b}{2} & = &
\mattwo{a}{3}{b}{2}\mattwo{2}{5}{1}{4} \\
\mattwo{2a+5b}{16}{a+4b}{11} & = & \mattwo{2a+3}{5a+12}{2b+2}{5b+8}.
\end{array}
\]
This equation can be rewritten as the system
\[
\begin{array}{rcl}
2a + 5b & = & 2a + 3 \\
16 & = & 5a + 12 \\
a + 4b & = & 2b + 2 \\
11 & = & 5b + 8 \end{array}
\]
which yields the solution $a = 4/5$ and $b = 3/5$.

\end{solution}
\end{exercise}

\begin{exercise} \label{c4.6.3}
Let
\[
A = \left(\begin{array}{rrr} 1 & 0 & -3\\ -2 & 1 & 1 \\ 0 & 1 & -5 \end{array}
\right).
\]
Let $A^t$ is the transpose of the matrix $A$, as defined in
Section~\ref{S:1.3}. Compute $AA^t$.

\begin{solution}

\[ AA^t = \matthree{1}{0}{-3}{-2}{1}{1}{0}{1}{-5}
\matthree{1}{-2}{0}{0}{1}{1}{-3}{1}{-5} =
\matthree{10}{-5}{15}{-5}{6}{-4}{15}{-4}{26}. \]



\end{solution}
\end{exercise}

\CEXER

\noindent In Exercises~\ref{c4.7.1a} -- \ref{c4.7.1c} decide for the
given pair of matrices $A$ and $B$ whether or not the products $AB$ or
$BA$ are defined and compute the products when possible.
\begin{exercise} \label{c4.7.1a}
\begin{matlabEquation}\label{MATLAB:26}
A=\left(\begin{array}{rrr} 2  &  2  & -2 \\ -4  &  4  &  0
\end{array}\right) \AND
B=\left(\begin{array}{rrr} 3 &  -2  &  0\\ 0 &  -1 &   4\\ -2 &  -3
&   5
\end{array}\right)
\end{matlabEquation}

\begin{solution}

Load the system into \Matlabp.  The matrix $AB$ is defined,
and typing {\tt A*B} yields:
\begin{verbatim}
ans =
    10     0    -2
   -12     4    16
\end{verbatim}
The matrix $BA$ is not defined, since $B$ has 3 columns while $A$
has 2 rows.  Typing {\tt B*A} generates an error message.

\end{solution}
\end{exercise}
\begin{exercise} \label{c4.7.1b}
\begin{matlabEquation}\label{MATLAB:27}
A=\left(\begin{array}{rrrrr}  -4  &  1  &  0  &  5  & -1\\
5  & -1  & -2  & -4  & -2\\ 1  &  5 &  -4   & 1  &  5
\end{array}\right) \AND
B=\left(\begin{array}{rrrrrr} 1  &  3  & -4  &  3  & -2  &  1\\
0  &  3  &  2  &  3  & -1  &  4\\ 5  &  4  &  4  &  5  & -1  &  0\\
-4  & -3  &  2  &  4  &  1  &  4
\end{array}\right)
\end{matlabEquation}

\begin{solution}
The matrix $AB$ is not defined because $A$ has 5 columns
while $B$ has four rows.  The matrix $BA$ is also not defined
because $B$ has 6 columns and $A$ has 3 rows.

\end{solution}
\end{exercise}
\begin{exercise} \label{c4.7.1c}
\begin{matlabEquation}\label{MATLAB:28}
A=\left(\begin{array}{rrrr}  -2  & -2  &  4  &  5\\
 0  & -3  & -4  &  3\\ 1  & -3  &  1  &  1\\ 0  &  1  &  0  &  4
\end{array}\right) \AND
B=\left(\begin{array}{rrrr} 2  &  3  & -4  &  5\\
4  & -3  &  0  & -2\\ -3 &  -4  & -4 &  -3\\ -2  & -2  &  3  & -1
\end{array}\right)
\end{matlabEquation}

\begin{solution}
Both $AB$ and $BA$ are defined and can be computed using
\Matlabp :
\begin{verbatim}
A*B                                     B*A
ans =                                   ans =   
   -34   -26     7   -23                    -8     4    -8    35
    -6    19    25    15                    -8    -1    28     3
   -15     6    -5     7                     2    27     0   -43
    -4   -11    12    -6                     7     0     3   -17
\end{verbatim}


\end{solution}
\end{exercise}



\end{document}
