\documentclass{ximera}
\input{../../preamble.tex}
\begin{document}

\noindent In Exercises~\ref{c6.8.2a} -- \ref{c6.8.2d}, find a $2\times 2$
matrix $C$ so that the given statement is satisfied.
\begin{exercise} \label{c6.8.2a}
The differential equation $\dot{X}=CX$ has a saddle at the origin with
unstable orbit in the direction $(2,3)$.

\begin{solution}

\ans One possible solution is $C = \mattwo{1}{0}{3}{-1}$.

\soln Since the system has an invariant manifold in the direction $(2,3)$,
$v_1 = (2,3)$.  Let $\lambda_1$ be the eigenvalue associated to $v_1$.
Since the manifold is unstable, $\lambda_1 > 0$.  The requirement
that the system has a saddle at the origin implies that $C$ has a second
eigenvalue $\lambda_2 < 0$.  Choose a second eigenvector $v_2$ independent
of $v_1$, such as $v_2 = (0,1)$ and choose eigenvalues, for example:
$\lambda_1 = 1$ and $\lambda_2 = -1$.

\para The matrix $C$ has two real eigenvalues.  Thus, by
Theorem~\ref{T:putinform}, $C$ is similar
to the diagonal matrix $D$ which has $\lambda_1$ and $\lambda_2$ as
entries along the main diagonal.  Therefore, $C = PDP^{-1}$, where $P$
is the matrix whose columns are the eigenvectors of $C$.  Thus,
\[
C = \mattwo{2}{0}{3}{1}\mattwo{1}{0}{0}{-1}\mattwo{\frac{1}{2}}{0}
{-\frac{3}{2}}{1} = \mattwo{1}{0}{3}{-1}. \]

\end{solution}
\end{exercise}
\begin{exercise} \label{c6.8.2b}
The differential equation $\dot{X}=CX$ has a spiral sink at the origin
where solutions decay to the origin at rate $\sigma=-0.5$.

\begin{solution}

\ans One possible matrix is $C = \mattwo{-0.5}{-1}{1}{-0.5}$.

\soln Since the origin is a spiral, the eigenvalues of $C$ are a complex
conjugate pair, $lambda_1 = \sigma + \tau i$ and $lambda_2 = \sigma -
\tau i$.  Since the origin is a sink, $\sigma$ is negative, and determines
the rate at which solutions decay to the origin, so $\sigma = -0.5$.
From Section~\ref{S:evchp}, we know that the matrix
\[ \mattwo{\sigma}{-\tau}{\tau}{\sigma} \]
has complex conjugate eigenvalues $\sigma \pm \tau$ if $\tau \neq 0$.
Thus, this matrix is a solution for any nonzero $\tau$.  For example,
let $\tau = 1$.

\end{solution}
\end{exercise}
\begin{exercise} \label{c6.8.2c}
The differential equation $\dot{X}=CX$ has an improper nodal source at the
origin with trajectories approaching the origin tangent to the $y$ axis.

\begin{solution}

\ans One possible matrix is $C = \mattwo{1}{0}{1}{1}$.

\soln Since the system has an improper nodal source at the origin, there
are two real equal positive eigenvalues, $\lambda_1 = \lambda_2 > 0$,
associated to a single eigenvector, $v$.  Let $\lambda = 1$ be an
eigenvalue.  The trajectories of an improper nodal system approach the
origin tangent to the eigenvector, so, since trajectories approach
tangent to the $y$-axis, the eigenvector is $v = (0,1)$.  By
Theorem~\ref{T:putinform}, if $C$ has one
real eigenvector, then $C = PDP^1$, where
\[ D = \mattwo{\lambda}{1}{0}{\lambda} \AND P = (v|w) \]
such that $Cv = v + \lambda w$.  We can assign an arbitrary value to
$w$.  For example, let $w = (1,0)$.  Then,
\[ C = \mattwo{0}{1}{1}{0}\mattwo{1}{1}{0}{1}\mattwo{0}{1}{1}{0} =
\mattwo{1}{0}{1}{1}. \]

\end{solution}
\end{exercise}
\begin{exercise} \label{c6.8.2d}
The differential equation $\dot{X}=CX$ has a nodal sink at the origin with
trajectories approaching the origin tangent to the line $y=x$.

\begin{solution}

\ans One possible matrix is $C = \mattwo{-1}{0}{1}{-2}$.

\soln Since the system has a nodal sink, the eigenvalues are real, unequal
and negative.  That is, $\lambda_2 < \lambda_1 < 0$.  The trajectories
of a nodal system approach the origin tangent to the eigenvector
associated to the eigenvalue with smaller absolute value.  Thus, for
this system, $v_1 = (1,1)$ is an eigenvalue associated to $\lambda_1$.
Arbitrarily assign values to $\lambda_1$, $\lambda_2$ and $v_2$, with
the given restrictions.  For example, let $\lambda_1 = -1$, $\lambda_2
= -2$ and $v_2 = (0,1)$.  Therefore, by
Theorem~\ref{T:putinform}, $C = PDP^{-1}$, where
\[ D = \mattwo{-1}{0}{0}{-2} \AND P = (v_1|v_2). \]
Thus,
\[ C = \mattwo{1}{0}{1}{1}\mattwo{-1}{0}{0}{-2}\mattwo{1}{0}{-1}{1} =
\mattwo{-1}{0}{1}{-2}. \]

\end{solution}
\end{exercise}
\end{document}
