\documentclass{ximera}
\input{../../preamble.tex}
\begin{document}
\begin{exercise} \label{c14.3.3}
Use reduction of order to find a solution to the equation
\begin{equation}  \label{e:inhomex2}
\ddot{x} + 3\dot{x}+2x = t.
\end{equation}
Compare the level of effort with the solution obtained using the
method of undetermined coefficients.

\begin{solution}
\ans A particular solution to the equation is given by
$x_p(t) = \frac{1}{2}(t-\frac{3}{2})$.

\soln The roots of the characteristic polynomial of the homogeneous
second order equation $\ddot x + 3\dot x + 2x = 0$
are $\lambda_1 = -1 $ and $\lambda_2 = -2$.
We choose $\lambda_1$ and $x_h(t)=e^{-t}$.  Then we find a solution
$y(t)$ of \eqref{eq:redeqreal}, that is,
\[
\frac{dy}{dt} = -(2\lambda_1 +a_1) y + e^{-\lambda_1 t}g(t) =
-y + te^t.
\]
This can be done by variation of parameters and we apply
Theorem~\ref{thm:varpar}.  Using the notation of this theorem, we can
choose
\[
H(t) = -t \AND c(t) = \int t e^{2t} dt = \frac{1}{2}e^{2t}(t-\frac{1}{2}),
\]
and obtain the solution
\[
y(t) = c(t)e^{H(t)} = \frac{1}{2}e^{t}(t-\frac{1}{2}).
\]
An integration of $y(t)$ now leads to the function $c(t)$ which is needed
for an application of Theorem~\ref{thm:redord}.  We compute
\[
c(t) = \int y(t)dt = \frac{e^t}{2}(t-\frac{3}{2}).
\]
Hence a particular solution is given by
\[
x_p(t) = c(t) x_h(t) =  \frac{1}{2}(t-\frac{3}{2}).
\]
Obviously the level of effort is much greater here than when using the method
of undetermined coefficients.  For a comparison, see the
beginning of Section~\ref{sec:2norderinhom} where
this problem is solved by undetermined coefficients.


\end{solution}
\end{exercise}
\end{document}
