\documentclass{ximera}
\input{../../preamble.tex}
\begin{document}
\begin{exercise} \label{c6.6.2}
Solve the initial value problem
\[
\frac{dX}{dt} = \mattwo{0}{1}{-2}{3} X
\]
where $X(0)=(2,1)^t$.

\begin{solution}

\ans The solution to the given initial value problem with $X(0) = (2,1)^t$
is
\[
X(t) = -3e^t\vectwo{1}{1} + e^{2t}\vectwo{1}{2}
= \cvectwo{e^{2t} - 3e^t}{2e^{2t} - 3e^t}.
\]

\soln Let \[ C = \mattwo{0}{1}{-2}{3}. \]
Then the solution to the system is $X(t) = e^{tC}X_0$, where
$X_0 = X(0) = (2,1)^t$.
To find $e^{tC}$, first find the eigenvalues of $C$ by solving
\[
0 = \lambda^2 - \trace(C) + \det(C) = (\lambda - 1)(\lambda - 2).
\]
The eigenvalues are $\lambda_1 = 1$ and $\lambda_2 = 2$.  We can
then find $e^{tC}$ using \eqref{E:exdist}:
\[
\begin{array}{rcl}
e^{tC} & = & \frac{1}{\lambda_2 - \lambda_1}(e^{\lambda_1 t}(C -
\lambda_2 I_2) - e^{\lambda_2 t}(C - \lambda_1 I_2)) \\
& = & e^t\left(\mattwo{0}{1}{-2}{3} - \mattwo{2}{0}{0}{2}\right) -
e^{2t}\left(\mattwo{0}{1}{-2}{3} - \mattwo{1}{0}{0}{1}\right) \\
& = &
e^t\mattwo{-2}{1}{-2}{1} - e^{2t}\mattwo{-1}{1}{-2}{2}.
\end{array}
\]
So, we can now compute
\[
X(t) = e^{tC}X_0
= \left(e^t\mattwo{-2}{1}{-2}{1} -
e^{2t}\mattwo{-1}{1}{-2}{2}\right)\vectwo{2}{1}.
\]
Complete the matrix multiplication to obtain $X(t)$.

\end{solution}
\end{exercise}
\end{document}
