\documentclass{ximera}
\input{../../preamble.tex}
\begin{document}

\noindent In Exercises~\ref{c14.2.6a} -- \ref{c14.2.6d} solve the given 
initial value problems by variation of parameters.
\begin{exercise}   \label{c14.2.6a}
$\dps \frac{dx}{dt} = t^2 x + t^2, \quad x(1)=1$.

\begin{solution}
\ans The solution to the initial value problem is
$x(t) = 2e^{\frac{1}{3}(t^3 - 1)} - 1$.

\soln By inspection $x(t) = -1$ is a solution to the inhomogeneous
equation.  The solution to the homogeneous equation $\dot{x}(t) = t^2x$ is
$x(t) = Ke^{H(t)}$, where
\[
H(t) = \int t^2dt = \frac{1}{3}t^3.
\]
So the general solution to the inhomogeneous equation is
\[
x(t) = Ke^{\frac{1}{3}t^3} - 1.
\]
Substitute the initial condition $x(1) = 1$ into this equation and
solve for $K = 2e^{-\frac{1}{3}}$.


\end{solution}
\end{exercise}
\begin{exercise}   \label{c14.2.6b}
$\dps \frac{dx}{dt} = x+2t, \quad x(0)=-1$.

\begin{solution}
\ans The solution to the initial value problem is
$x(t) = e^t - 2t - 2$.

\soln The solution to the homogeneous equation $\dot{x}=x$ is $x(t)=ce^t$
for some constant $c$.  The method of variation of parameters looks for 
solutions to the inhomogeneous equation of the form $x(t)=c(t)e^t$.  If this 
$x(t)$ is a solution to the inhomogeneous equation $\dot{x}=x+2t$, then
\[
x+2t=\dot{x}=\dot{c}e^t+ce^t = \dot{c}e^t+x.
\]
Therefore,
\[
\dot{c} = 2te^{-t}.
\]
Integrating by parts yields
\[
c(t) = 2\int te^{-t}dt = -2(t+1)e^{-t} + K.
\]
Thus the general solution to the inhomogeneous equation is:
\[
x(t) = -2(t+1) + Ke^t.
\]
Using the initial condition $x(0)=-1$ yields $K=1$. 

\end{solution}
\end{exercise}
\begin{exercise}   \label{c14.2.6c}
$\dps \frac{dx}{dt} = 
\frac{t}{t^2+1}x+\sin(t)\sqrt{t^2+1},\quad x(0)=2$.

\begin{solution}
\ans The solution to the initial value problem is
$x(t) = (3 - \cos t)\sqrt{t^2 + 1}$.

\soln By Theorem~\ref{thm:varpar}, the
solution to the initial value problem is $x(t) = c(t)e^{H(t)}$, where
$\frac{dx}{dt} = a(t)x + g(t)$.  So
\[
H(t) = \int_{t_0}^t a(\tau)d\tau = \int_0^t\frac{\tau}{\tau^2 + 1}d\tau
= \ln\sqrt{t^2 + 1}.
\]
\[
c(t) = \int_{t_0}^t g(\tau)e^{-H(\tau)}d\tau + x_0
= \int_0^t \sin(\tau)d\tau + 2
= 3 - \cos t.
\]

\end{solution}
\end{exercise}
\begin{exercise}   \label{c14.2.6d}
$\dps \frac{dx}{dt} = 2x+\frac{1}{t}e^{2t}, \quad x(1)=4$.

\begin{solution}
\ans The solution to the initial value problem is
\[
x(t) = e^{2t}(4e^{-2}+\ln t).
\]

\soln The solution to the homogeneous equation $\dot{x}=2x$ is $x(t)=e^{2t}$.
 Using variation of parameters we look for a solution to the inhomogeneous
equation $\dot{x}=2x+\frac{1}{t}e^{2t}$ of the form $x(t)=c(t)e^{2t}$.  If
$x(t)$ is a solution to the inhomogeneous equation, then
\[
2x+\frac{1}{t}e^{2t} =\dot{x}=\dot{c}e^{2t}+2ce^{2t} = \dot{c}e^{2t}+2x.
\]
Therefore, 
\[
\dot{c} = \frac{1}{t},
\]
and 
\[
c(t) = \ln|t| + K.
\]
The general solution to the inhomogeneous equation is:
\[
x(t) = (\ln|t| + K)e^{2t}.
\]
Using the initial condition $x(1)=4$, we find that $K=4e^{-2}$.



\end{solution}
\end{exercise}
\end{document}
