\documentclass{ximera}
\input{../../preamble.tex}
\begin{document}
\begin{exercise} \label{c11.1.2}
Find the solution to the system
\begin{eqnarray*}
\dot{x}_1 & = & -2x_1+x_2+x_3 \\
\dot{x}_2 & = & -x_1-2x_2+x_4 \\
\dot{x}_3 & = & -2x_3+x_4 \\
\dot{x}_4 & = & -x_3-2x_4
\end{eqnarray*}
satisfying $X_0=(1,2,-1,-3)^t$.

\begin{solution}
\ans
\[
X(t) = e^{-2t}
\left(\begin{array}{c}
\cos t + 2\sin t - t(\cos t + 3\sin t) \\
2\cos t - \sin t + t(\sin t - 3\cos t) \\
-\cos t - 3\sin t \\
-\sin t - 3\cos t
\end{array}\right).
\]

\soln Write the system as $\dot{X} = AX$, where
\[
A =
\left(\begin{array}{rrrr}
-2 & 1 & 1 & 0 \\
-1 & -2 & 0 & 1 \\
0 & 0 & -2 & 1 \\
0 & 0 & -1 & -2
\end{array}\right).
\]
Note that $A$ is in Jordan normal form and has a double complex conjugate
eigenvalue at $\lambda = -2 \pm i$.  We can write $A = J + M$, where
\[
J = 
\left(\begin{array}{rr|rr}
-2 & 1 & 0 & 0 \\
-1 & -2 & 0 & 0 \\
\hline
0 & 0 & -2 & 1 \\
0 & 0 & -1 & -2
\end{array}\right) \AND
M =
\left(\begin{array}{rr|rr}
0 & 0 & 1 & 0 \\
0 & 0 & 0 & 1 \\
\hline
0 & 0 & 0 & 0 \\
0 & 0 & 0 & 0
\end{array}\right).
\]
Since $J$ and $M$ commute, we can compute the closed form solution to the
system, using $\sigma = -2$ and $\tau = -1$:
\[
\begin{array}{rcl}
X(t) & = & e^{tA}X_0 \\
& = & e^{tJ}e^{tM}X_0 \\
& = & e^{-2t}\left(\begin{array}{rr|rr}
\cos t & \sin t & 0 & 0 \\
-\sin t & \cos t & 0 & 0 \\
\hline
0 & 0 & \cos t & \sin t \\
0 & 0 & -\sin t & \cos t
\end{array}\right)
\left(\begin{array}{rr|rr}
1 & 0 & t & 0 \\
0 & 1 & 0 & t \\
\hline
0 & 0 & 1 & 0 \\
0 & 0 & 0 & 1
\end{array}\right)X_0 \\
& = & e^{-2t}
\left(\begin{array}{rr|rr}
\cos t & \sin t & t\cos t & t\sin t \\
-\sin t & \cos t & -t\sin t & t\cos t \\
\hline
0 & 0 & \cos t & \sin t \\
0 & 0 & -\sin t & \cos t
\end{array}\right)
\left(\begin{array}{r} 1 \\ 2 \\ -1 \\ -3 \end{array}\right).
\end{array}
\]

\end{solution}
\end{exercise}
\end{document}
