\documentclass{ximera}
\input{../../preamble.tex}
\begin{document}
\begin{exercise} \label{c11.1.3}
Let $X(t)$ be the solution to 
\[
\frac{dX}{dt} = \left(\begin{array}{rrr} 
-\half & 1 & 0 \\ 0 & -\half & 1\\ 0 & 0 & -\half
\end{array}\right)X
\]
satisfying $X_0=(0,1,1)^t$. Show that $X(2)$ is further from the 
origin than $X(0)$.

\begin{solution}
\ans $X(t) = \cvecthree{t + \frac{1}{2}t^2}{1 + t}{1}$. The distance from $X(0)$ to the 
origin is $\sqrt{2} \approx 1.4142$ and the distance from $X(2)$ to the origin is
$e^{-1}\sqrt{26} \approx 1.8758$.

\soln Let $B$ be the matrix of this system.  Note that $B$ is a single Jordan block
with a triple eigenvalue at $\lambda = -\frac{1}{2}$, and that we can write
$B = -\frac{1}{2}I_3 + N$, where $N$ is the matrix with entries $1$ on the
superdiagonal.  Then, since $I_3$ and $N$ commute, we can write:
\[
\begin{array}{rcl}
X(t) & = & e^{tB}X_0 \\
& = & e^{\lambda tI_3}e^{tN}X_0 \\
& = & e^{\lambda t}(I_3 + tN + \frac{1}{2}t^2N^2)X_0 \\
& = & e^{-\frac{1}{2} t}\cmatthree{1}{t}{\frac{1}{2}t^2}{0}{1}{t}{0}{0}{1}
\vecthree{0}{1}{1} \\
& = & \cvecthree{t + \frac{1}{2}t^2}{1 + t}{1}.
\end{array}
\]
Next, compute $X(2) = e^{-1}(4,3,1)^t$.
The distance from $X(0)$ to the origin is $\sqrt{0 + 1 + 1} = \sqrt{2}
\approx 1.4142$.  The distance from $X(2)$ to the origin is
$e^{-1}\sqrt{4^2 + 3^2 + 1} = e^{-1}\sqrt{26} \approx 1.8758$.
Thus, $X(2)$ is indeed further from the origin than $X(0)$.

\end{solution}
\end{exercise}
\end{document}
