\documentclass{ximera}
\input{../../preamble.tex}
\begin{document}

\TEXER

\noindent In Exercises~\ref{c14.3.1a} -- \ref{c14.3.1b} solve the given 
initial value problems by variation of parameters.

\begin{exercise}  \label{c14.3.1a}
\[
\frac{dX}{dt}=\frac{1}{2}\mattwo{1}{1}{1}{1} X + \vectwo{e^t}{0},\quad
X(0) = \vectwo{1}{-1}.
\]

\begin{solution}
\ans The solution to the initial value problem is
\[
X(t) = \frac{1}{2}\cvectwo{te^t + e^t + 1}{te^t - e^t - 1}.
\]

\soln This system can be written as $\dot{X} = AX + G(t)$, where
\[
A = \frac{1}{2}\mattwo{1}{1}{1}{1} \AND G(t) = \vectwo{e^t}{0}.
\]
We can then solve the system by variation of parameters, as described in
Theorem~\ref{thm:varparsys}:

\paragraph{Step 1.} The eigenvalues of $A$ are $\lambda_1 = 0$ and
$\lambda_2 = 1$, with associated eigenvectors $v_1 = (1,-1)^t$ and
$v_2 = (1,1)^t$.  Thus, a basis of solutions to the homogeneous system
$\dot{X} = AX$ is
\[
X_1(t) = \vectwo{1}{-1} \AND X_2(t) = e^t\vectwo{1}{1}.
\]
\paragraph{Step 2.} To compute the vector $D(t)$, first compute
\[
Y(t)^{-1} = (X_1(t)|X_2(t))^{-1} = \cmattwo{1}{e^t}{-1}{e^t}^{-1} =
\frac{1}{2e^t}\cmattwo{e^t}{-e^t}{1}{1} =
\frac{1}{2}\cmattwo{1}{-1}{e^{-t}}{e^{-t}}.
\]
Then,
\[
D(t) = Y(t)^{-1}G(t) =
\frac{1}{2}\cmattwo{1}{-1}{e^{-t}}{e^{-t}}\vectwo{e^t}{0} =
\frac{1}{2}\vectwo{e^{t}}{1}.
\]
\paragraph{Step 3.} We find $c_1(0)$ and $c_2(0)$ using the initial
condition
\[
X_0 = c_1(0)X_1(0) + c_2(0)X_2(0).
\]
Therefore,
\[
\vectwo{1}{-1} = c_1(0)\vectwo{1}{-1} + c_2(0)\vectwo{1}{1}.
\]
Solve this system to obtain $c_1(0) = 1$ and $c_2(0) = 0$.  By definition,
$\dot{c_j} = d_j$.  Thus,
\[
c_1(t) = \int_{t_0}^td_1(\tau)d\tau + c_1(0)
= \frac{1}{2}\int_0^te^\tau d\tau + 1 = \frac{1}{2}(e^t + 1).
\]
\[
c_2(t) = \int_{t_0}^td_2(\tau)d\tau + c_2(0)
= \frac{1}{2}\int_0^td\tau = \frac{t}{2}.
\]
\paragraph{Step 4.} So, the solution to the initial value problem is
\[
X(t) = c_1(t)X_1(t) + c_2(t)X_2(t)
= \frac{1}{2}\left((e^t + 1)\vectwo{1}{-1} + \frac{t}{2}e^t\vectwo{1}{1}
\right).
\]

\end{solution}
\end{exercise}
\begin{exercise}  \label{c14.3.1b}
\[
\frac{dX}{dt}=\mattwo{1}{3}{3}{1} X + \vectwo{2t}{t},\quad
X(0) = \vectwo{0}{1}.
\]

\begin{solution}
\ans The solution to the given initial value problem is
\[
X(t) = \frac{1}{32}\cvectwo{19e^{4t} - 12e^{-2t} - 4t - 7}
{19e^{4t} + 12e^{-2t} - 20t + 1}.
\]
\soln This system can be written as $\dot{X} = AX + G(t)$, where
\[
A = \mattwo{1}{3}{3}{1} \AND G(t) = \vectwo{2t}{t}.
\]
We can then solve the system by variation of parameters, as described in
Theorem~\ref{thm:varparsys}:

\paragraph{Step 1.} The eigenvalues of $A$ are $\lambda_1 = -2$ and
$\lambda_2 = 4$, with associated eigenvectors $v_1 = (1,-1)^t$ and
$v_2 = (1,1)^t$.  Thus, a basis of solutions to the homogeneous system
$\dot{X} = AX$ is
\[
X_1(t) = e^{-2t}\vectwo{1}{-1} \AND X_2(t) = e^{4t}\vectwo{1}{1}.
\]
\paragraph{Step 2.} To compute the vector $D(t)$, first compute
\[
Y(t)^{-1} = \cmattwo{e^{-2t}}{e^{4t}}{-e^{-2t}}{e^{4t}}^{-1}
= \frac{1}{2e^{2t}}\cmattwo{e^{4t}}{-e^{4t}}{e^{-2t}}{e^{-2t}}
= \frac{1}{2}\cmattwo{e^{2t}}{-e^{2t}}{e^{-4t}}{e^{-4t}}.
\]
Then,
\[
D(t) = Y(t)^{-1}G(t) =
\frac{1}{2}\cmattwo{e^{2t}}{-e^{2t}}{e^{-4t}}{e^{-4t}}\vectwo{2t}{t} =
\frac{1}{2}\vectwo{te^{2t}}{3te^{-4t}}.
\]
\paragraph{Step 3.} We find $c_1(0)$ and $c_2(0)$ using the initial
condition
\[
X_0 = c_1(0)X_1(0) + c_2(0)X_2(0).
\]
Therefore,
\[
\vectwo{0}{1} = c_1(0)\vectwo{1}{-1} + c_2(0)\vectwo{1}{1}.
\]
Solve this system to obtain $c_1(0) = -\frac{1}{2}$ and $c_2(0) =
\frac{1}{2}$.  By definition, $\dot{c_j} = d_j$.  Thus,
\[
c_1(t) = \int_{t_0}^td_1(\tau)d\tau + c_1(0)
= \frac{1}{2}\int_0^t \tau e^{2\tau}d\tau - \frac{1}{2}
= \frac{1}{8}(2te^{2t} - e^{2t} - 3).
\]
\[
c_2(t) = \int_{t_0}^td_2(\tau)d\tau + c_2(0)
= \frac{3}{2}\int_0^t \tau e^{-4\tau}d\tau + \frac{1}{2}
= \frac{1}{32}(-4te^{-4t} - e^{-4t} + 19).
\]

\paragraph{Step 4.} So, the solution to the initial value problem is
\[
X(t) = c_1(t)X_1(t) + c_2(t)X_2(t)
= \frac{1}{8}(2t - 1 - 3e^{-2t})\vectwo{1}{-1} +
\frac{1}{32}(-4t - 1 + 19e^{4t})\vectwo{1}{1}.
\]


\end{solution}
\end{exercise}
\end{document}
