\documentclass{ximera}
\input{../../preamble.tex}
\begin{document}
\begin{exercise}  \label{c17.3.4}
Find the general solution to the system of differential equations
\[
\frac{dX}{dt}= \mattwoc{0}{1}{\frac{3}{t^2}}{\frac{1}{t}}X+\vectwoc{t}{2t}.
\]
{\bf Hint:} Verify that 
\[
X_1(t) = \vectwoc{t^3}{3t^2}\AND X_2(t) = \vectwoc{\frac{1}{t}}{-\frac{1}{t^2}}
\]
are solutions to the homogeneous equation and then use variation of parameters.

\begin{solution}

\ans $X(t) = \left(\alpha_1+\frac{1}{4}\left(2\ln t -
\frac{1}{t}\right)\right)X_1(t) + \left(\alpha_2 + \frac{1}{8}
\left(2t^3-t^4\right)\right)X_2(t)$.

\soln  Begin by verifying that $X_1=(t^3,3t^2)^t$ and 
$X_2=(\frac{1}{t},-\frac{1}{t^2})^t$ solve the homogeneous
equation
\[
\frac{dX}{dt}= \cmattwo{0}{1}{\frac{3}{t^2}}{\frac{1}{t}}X.
\]
That is,
\[
\dot{X}_1 = \cvectwo{3t^2}{6t} \AND 
\mattwo{0}{1}{\frac{3}{t^2}}{\frac{1}{t}}\cvectwo{t^3}{3t^2} = 
\cvectwo{3t^2}{3t+3t} = \cvectwo{3t^2}{6t}
\]
and 
\[
\dot{X}_2 = \vectwo{-\frac{1}{t^2}}{\frac{2}{t^3}} \AND 
\mattwo{0}{1}{\frac{3}{t^2}}{\frac{1}{t}}
\vectwo{\frac{1}{t}}{-\frac{1}{t^2}} = 
\cvectwo{-\frac{1}{t^2}}{\frac{3}{t^3}-\frac{1}{t^3}} 
= \vectwo{-\frac{1}{t^2}}{\frac{2}{t^3}}
\]

Next we look for a particular solution to the inhomogeneous equation of 
the form $X(t)=c_1(t)X_1(t)+c_2(t)X_2(t)$.  Equation~\eqref{e:D(t)} in
Theorem~\ref{thm:varparsys} states that $c_j$ satisfies
\[
\vectwo{\dot{c}_1}{\dot{c}_2} = (X_1|X_2)\inv \vectwo{t}{2t}.
\]
Now 
\[
 (X_1|X_2)\inv = \mattwo{t^3}{\frac{1}{t}}{3t^2}{-\frac{1}{t^2}}\inv = 
\frac{1}{4t}\mattwo{\frac{1}{t^2}}{\frac{1}{t}}{3t^2}{-t^3}
\]
It follows that 
\begin{eqnarray*}
\dot{c}_1 & = & \frac{1}{4}\left(\frac{1}{t^2}+\frac{2}{t}\right) \\
\dot{c}_2 & = & \frac{1}{4}\left(3t^2-2t^3\right).
\end{eqnarray*}
Integration yields
\begin{eqnarray*} 
c_1 & = & \frac{1}{4}\left(2\ln t - \frac{1}{t}\right)\\
c_2 & = & \frac{1}{8}\left(2t^3-t^4\right).
\end{eqnarray*}
Adding the general solution to the homogeneous equation to the specific
solution to the inhomogeneous equation yields the general solution to the
inhomogeneous equation.



\end{solution}
\end{exercise}
\end{document}
