\documentclass{ximera}
\input{../../preamble.tex}
\begin{document}
\begin{exercise}  \label{c6.6.05}
Justify Euler's formula \eqref{E:Euler} as follows.  Recall the
Taylor series
\begin{eqnarray*}
e^x & = & 1 + x + \frac{1}{2!}x^2 + \cdots + \frac{1}{n!}x^n + \cdots\\
\cos x & = & 1 - \frac{1}{2!}x^2 + \frac{1}{4!}x^4 + \cdots +
(-1)^n \frac{1}{(2n)!}x^{2n} + \cdots \\
\sin x & = & x - \frac{1}{3!}x^3 + \frac{1}{5!}x^5 + \cdots +
(-1)^n \frac{1}{(2n+1)!}x^{2n+1} + \cdots.
\end{eqnarray*}
Now evaluate the Taylor series $e^{i\theta}$ and separate into real and
imaginary parts.

\begin{solution}

Using the identities $i^2 = -1$, $i^3 = -i$, and $i^4 = 1$, write
the Taylor series:
\[
\begin{array}{rcl}
e^{i\theta} & = & 1 + i\theta + \frac{1}{2!}(i\theta)^2 +
\frac{1}{3!}(i\theta)^3 + \frac{1}{4!}(i\theta)^4 +
\frac{1}{5!}(i\theta)^5 + \cdots \\
& = & 1 + i\theta - \frac{1}{2!}\theta^2 - \frac{1}{3!}i\theta^3 +
\frac{1}{4!}\theta^4 + \frac{1}{5!}i\theta^5 + \cdots \\
& = & (1 - \frac{1}{2!}\theta^2 + \frac{1}{4!}\theta^4 - \cdots)
+ i(\theta - \frac{1}{3!}\theta^3 + \frac{1}{5!}\theta^5 - \cdots) \\
& = & \cos\theta + i\sin\theta. \end{array}
\]


\end{solution}
\end{exercise}
\end{document}
